1. several helper lemmas for preservation theroem
2. preservation theorem finished.

3. soundness theorem stated and proved.

4. One useful lemma to be finished: reduction preserve well-formness of heap and stack. Working on it now.

CIFC.v
@@ -51,13 +51,12 @@ Inductive tm : Type :=
 
 (* special terms *)
   | ObjId: oid -> tm
-  | NPE : tm
   (* runtime labeled date*)
   | v_l : tm -> Label -> tm
   | v_opa_l : tm -> Label -> tm.
 
 Inductive method_def : Type :=
-  | m_def : cn -> id -> cn -> id -> tm -> tm -> method_def.
+  | m_def : cn -> id -> cn -> id -> tm -> method_def.
 
 
 Inductive CLASS : Type :=
@@ -80,9 +79,6 @@ Inductive value : tm -> Prop :=
   | v_opa_labeled : forall v lb,
      (* value v ->*)
       value (v_opa_l v lb).
-
-Inductive Exception : tm -> Prop :=
-  | exception : Exception NPE.
 
 (* stack frame *)
 Definition stack_frame : Type := id -> (option tm).
@@ -172,10 +168,6 @@ Definition beq_oid x y :=
 Inductive Sigma := 
   | SIGMA : stack -> heap -> Sigma.
 
-Definition Config := pair Sigma tm. 
-
-Check Config.
-
 Definition get_stack (sgm : Sigma) : stack :=
   match sgm with
    | SIGMA s h => s
@@ -215,7 +207,7 @@ Fixpoint find_method_body (methods : list method_def) (m : id) :=
   match methods with
     | nil => None
     | h :: t =>  match h with 
-                  | m_def cls m' cls_a arg_id body retV => if beq_id m m' then Some (m_def cls m' cls_a arg_id body (Return retV)) else find_method_body t m
+                  | m_def cls m' cls_a arg_id body => if beq_id m m' then Some (m_def cls m' cls_a arg_id  (Return body)) else find_method_body t m
                  end
   end.
 
@@ -248,20 +240,30 @@ Check init_field_map.
 Definition add_heap_obj (h : heap) (o : oid) (ho : heapObj) :=
   fun x' => if beq_oid o x' then (Some ho) else h x'.
 
-Inductive step : tm -> Sigma -> tm -> Sigma -> Prop :=
+
+Inductive config := 
+  | Config : tm -> Sigma -> config
+  | Error_state : config.
+Hint Constructors config.
+
+Reserved Notation "c '==>' c'"
+  (at level 40, c' at level 39).
+
+
+Inductive reduction : config -> config -> Prop :=
 (* variabel access *)
   | ST_var : forall id sigma s h lb sf lsf v s',
       sigma = SIGMA s h ->
       s = cons lsf s' ->
       lsf = Labeled_frame lb sf ->
       Some v = sf(id) ->
-      (Tvar id) / sigma ==> v / sigma
+      Config (Tvar id) sigma ==> Config v sigma
 
 (* field read *)
   (* context rule *)
   | ST_fieldRead1 : forall sigma sigma' e e' f,
-       e / sigma ==>  e' / sigma' -> 
-      (FieldAccess e f) / sigma ==> (FieldAccess e' f) / sigma'
+      Config e sigma ==>  Config e' sigma' -> 
+      Config (FieldAccess e f) sigma ==> Config (FieldAccess e' f) sigma'
   (* normal field access *)
   | ST_fieldRead2 : forall sigma sigma' o s h fname lb cls fields v l' s',
       sigma = SIGMA s h ->
@@ -269,28 +271,33 @@ Inductive step : tm -> Sigma -> tm -> Sigma -> Prop :=
       Some v = fields(fname) -> 
       l' = join_label lb (current_label sigma) ->
       s' = update_current_label s l'-> 
-      sigma' = SIGMA s' (get_heap sigma) ->
-      (FieldAccess (ObjId o) fname) / sigma ==> v / sigma'
+      sigma' = SIGMA s' h ->
+      Config (FieldAccess (ObjId o) fname) sigma ==> Config v sigma'
   (* null pointer exception for field access *)
   | ST_fieldReadException : forall sigma f ,
-      (FieldAccess null f) / sigma ==> NPE / sigma
+      Config (FieldAccess null f) sigma ==> Error_state
+  | ST_fieldRead3 : forall sigma e f,
+      Config e sigma ==>  Error_state -> 
+      Config (FieldAccess e f) sigma ==> Error_state
+
+
 
 (* method call *)
   (* context rule: evaluate object target *)
   | ST_MethodCall1 : forall sigma sigma' e e' e2 id,
-       e / sigma ==>  e' / sigma' -> 
-      (MethodCall e id e2) / sigma ==> (MethodCall e' id e2) / sigma'
+       Config e sigma ==>  Config e' sigma' -> 
+      Config (MethodCall e id e2) sigma ==> Config (MethodCall e' id e2)  sigma'
   (* context rule: evaluate arguments *)
   | ST_MethodCall2 : forall sigma sigma' v e e' id,
       (forall t, value t -> t<> null -> e <> unlabelOpaque t) ->
-      e / sigma ==>  e' / sigma' -> 
+      Config e sigma ==>  Config e' sigma' -> 
       value v ->
-      (MethodCall v id e) / sigma ==> (MethodCall v id e') / sigma'
+      Config (MethodCall v id e) sigma ==> Config (MethodCall v id e') sigma'
   (* normal method call *)
-  | ST_MethodCall3 : forall sigma sigma' o s h cls fields v lx l theta s' sf lsf arg_id cls_a body meth returnT return_v,
+  | ST_MethodCall3 : forall sigma sigma' o s h cls fields v lx l theta s' sf lsf arg_id cls_a body meth returnT,
       sigma = SIGMA s h ->
       Some (Heap_OBJ cls fields lx) = h(o) -> 
-      Some (m_def returnT meth cls_a arg_id body (Return return_v)) = find_method cls meth -> 
+      Some (m_def returnT meth cls_a arg_id (Return body)) = find_method cls meth -> 
       value v ->
       sf = sf_update (sf_update empty_stack_frame (Id "this") (ObjId o)) arg_id v ->
       l = (current_label sigma) ->
@@ -298,109 +305,150 @@ Inductive step : tm -> Sigma -> tm -> Sigma -> Prop :=
       theta = lsf -> 
       s' = cons theta s ->
       sigma' = SIGMA s' (get_heap sigma) ->
-      MethodCall (ObjId o) meth v / sigma ==> (Sequence body (Return return_v)) / sigma'
+      Config (MethodCall (ObjId o) meth v) sigma ==>  Config (Return body) sigma'
   (* null pointer exception for method call *)
   | ST_MethodCallException : forall sigma v meth, 
-      MethodCall null meth v / sigma ==> NPE / sigma
+      Config (MethodCall null meth v) sigma ==> Error_state
+  (* context rule error 1*)
+  | ST_MethodCall4 : forall sigma e e2 id,
+       Config e sigma ==>  Error_state -> 
+      Config (MethodCall e id e2) sigma ==> Error_state
+  (* context rule error 2*)
+  | ST_MethodCall5 : forall sigma v e id,
+      (forall t, value t -> t<> null -> e <> unlabelOpaque t) ->
+      Config e sigma ==>  Error_state -> 
+      value v ->
+      Config (MethodCall v id e) sigma ==> Error_state
+
 
 (* method call with unlabel opaque *)
-  | ST_MethodCall_unlableOpaque : forall sigma sigma' o s h cls fields v lx l' lb s' sf lsf arg_id cls_a body meth returnT return_v,
+  | ST_MethodCall_unlableOpaque : forall sigma sigma' o s h cls fields v lx l' lb s' sf lsf arg_id cls_a body meth returnT,
       sigma = SIGMA s h ->
       Some (Heap_OBJ cls fields lx) = h(o) -> 
       sf = sf_update (sf_update empty_stack_frame (Id "this") (ObjId o)) arg_id v ->
       l' = join_label lb (current_label sigma) ->
       lsf = Labeled_frame l' sf ->
       s' = cons lsf s ->
-      Some (m_def returnT meth cls_a arg_id body (Return return_v)) = find_method cls meth ->
+      Some (m_def returnT meth cls_a arg_id  (Return body)) = find_method cls meth ->
       sigma' = SIGMA s' (get_heap sigma) ->
-      MethodCall (ObjId o) meth (unlabelOpaque (v_opa_l v lb)) / sigma ==> (Sequence body (Return return_v)) / sigma'
+      Config (MethodCall (ObjId o) meth (unlabelOpaque (v_opa_l v lb)))  sigma ==>Config (Return body) sigma'
 
   (* null pointer exception for method call with unlabel opaque of null data*)
   | ST_MethodCallOpaqueDataException : forall sigma o meth, 
-      MethodCall (ObjId o) meth (unlabelOpaque null) / sigma ==> NPE / sigma
+      Config (MethodCall (ObjId o) meth (unlabelOpaque null)) sigma ==> Error_state
 
 (* new expression *)
-  | ST_NewExp : forall sigma sigma' F o h cls h' s lb cn,
+  | ST_NewExp : forall sigma sigma' F o h cls h' s lb cls_name field_defs method_defs,
       sigma = SIGMA s h->
       h(o) = None -> 
+      cls = (class_def cls_name field_defs method_defs) ->
       F =  (init_field_map (find_fields cls) empty_field_map) ->
       lb = (current_label sigma) -> 
-
       h' = add_heap_obj h o (Heap_OBJ cls F lb) ->
       sigma' = SIGMA s h' ->
-      NewExp cn / sigma ==> ObjId o / sigma'
+      Config (NewExp cls_name) sigma ==> Config (ObjId o) sigma'
 
 
 (* label data express *)
   (* context rule *)
   | ST_LabelData1 : forall sigma sigma' e e' lb,
-       e / sigma ==>  e' / sigma' -> 
-      (labelData e lb) / sigma ==> (labelData e' lb) / sigma'
+      Config e sigma ==>  Config e' sigma' -> 
+      Config (labelData e lb) sigma ==> Config (labelData e' lb) sigma'
   (* label data *)
   | ST_LabelData2 : forall sigma v lb,
       value v ->
-      (labelData v lb) / sigma ==> (v_l v lb) / sigma
+      Config (labelData v lb) sigma ==>  Config (v_l v lb)  sigma
   (* label data exception *)
   | ST_LabelDataException : forall sigma lb,
-      (labelData null lb) / sigma ==> NPE / sigma
+      Config (labelData null lb) sigma ==> Error_state
+  (* context rule error*)
+  | ST_LabelDataError : forall sigma e lb,
+      Config e sigma ==>  Error_state -> 
+      Config (labelData e lb) sigma ==> Error_state
+
+
+
 
 (* unlabel *)
   (* context rule *)
   | ST_unlabel1 : forall sigma sigma' e e',
-       e / sigma ==>  e' / sigma' -> 
-      (unlabel e) / sigma ==> (unlabel e') / sigma'
+      Config e sigma ==>  Config e' sigma' -> 
+      Config  (unlabel e) sigma ==> Config (unlabel e') sigma'
   (* unlabel *)
   | ST_unlabel2 : forall sigma v lb l' sigma' s h s',
       sigma = SIGMA s h ->
       l' = join_label lb (current_label sigma) ->
       s' = update_current_label s l'-> 
       sigma' = SIGMA s' (get_heap sigma) ->
-      (unlabel (v_l v lb)) / sigma ==> v / sigma'
+      Config (unlabel (v_l v lb)) sigma ==> Config v sigma'
   (* unlabel data exception *)
   | ST_unlabelDataException : forall sigma,
-      (unlabel null) / sigma ==> NPE / sigma
+      Config (unlabel null) sigma ==> Error_state
+  (* context rule error*)
+  | ST_unlabelContextError : forall sigma  e,
+      Config e sigma ==>  Error_state -> 
+      Config  (unlabel e) sigma ==> Error_state
+
 
 (* Label of *)
   (* context rule *)
   | ST_labelof1 : forall sigma sigma' e e',
-       e / sigma ==>  e' / sigma' -> 
-       (labelOf e) / sigma ==> (labelOf e') / sigma'
+       Config e sigma ==>  Config e' sigma' -> 
+       Config (labelOf e) sigma ==> Config (labelOf e') sigma'
   (* label of  *)
   | ST_labelof2 : forall sigma v lb,
-      (labelOf (v_l v lb)) / sigma ==> l lb / sigma
+      Config (labelOf (v_l v lb)) sigma ==> Config (l lb) sigma
   | ST_labelOfDataException : forall sigma, 
-      labelOf null / sigma ==> NPE / sigma
-
+      Config (labelOf null) sigma ==> Error_state
+  (* context rule error*)
+  | ST_labelofCtxError : forall sigma e,
+       Config e sigma ==>  Error_state -> 
+       Config (labelOf e) sigma ==> Error_state
 
 (* unlabel opaque*)
   (* context rule *)
   | ST_unlabel_opaque1 : forall sigma sigma' e e',
-       e / sigma ==>  e' / sigma' -> 
-      (unlabelOpaque e) / sigma ==> (unlabelOpaque e') / sigma'
+      Config e sigma ==>  Config e' sigma' -> 
+     Config (unlabelOpaque e) sigma ==>  Config (unlabelOpaque e') sigma'
+  (* context rule error*)
+  | ST_unlabel_opaque_ctx_error : forall sigma e,
+      Config e sigma ==>  Error_state -> 
+     Config (unlabelOpaque e) sigma ==>  Error_state
   (* unlabel opaque *)
   | ST_unlabel_opaque2 : forall sigma v lb l' sigma' s h s',
       sigma = SIGMA s h ->
       l' = join_label lb (current_label sigma) ->
       s' = update_current_label s l'-> 
       sigma' = SIGMA s' (get_heap sigma) ->
-      (unlabelOpaque (v_opa_l v lb)) / sigma ==> v / sigma'
+      Config (unlabelOpaque (v_opa_l v lb)) sigma ==> Config v sigma'
   | ST_unlabel_opaqueDataException : forall sigma, 
-      unlabelOpaque null / sigma ==> NPE / sigma
+      Config (unlabelOpaque null) sigma ==> Error_state
 
 (* Opaque call *)
   (* context rule *)
   | ST_opaquecall1 : forall sigma sigma' e e',
        (forall v, value v -> e <> Return v) ->
-       e / sigma ==>  e' / sigma' -> 
-      (opaqueCall e) / sigma ==> (opaqueCall e') / sigma'
+       Config e sigma ==>  Config e' sigma' -> 
+      Config (opaqueCall e) sigma ==> Config (opaqueCall e') sigma'
+  (* context rule error*)
+  | ST_opaquecall_ctx_error : forall sigma e,
+      Config e sigma ==>  Error_state -> 
+     Config  (opaqueCall e) sigma  ==>  Error_state
   (* return context rule*)
   | ST_opaquecall_return1 : forall sigma sigma' e e',
-       e / sigma ==>  e' / sigma' -> 
-      (opaqueCall (Return e)) / sigma ==> (opaqueCall (Return e')) / sigma'
-  (* opaque call with value, without method call inside*)
-  | ST_opaquecall_val2 : forall sigma v,
+       Config e sigma ==> Config  e' sigma' -> 
+      Config (opaqueCall (Return e)) sigma ==> Config (opaqueCall (Return e')) sigma'
+  (* return context rule error*)
+  | ST_opaquecall_return_error : forall sigma e,
+       Config e sigma ==> Error_state -> 
+      Config (opaqueCall (Return e)) sigma ==> Error_state
+
+
+  (* opaque call with value, without method call inside *)
+  | ST_opaquecall_val2 : forall sigma v lb,
       (value v) ->
-      (opaqueCall v) / sigma ==> v / sigma
+      lb = (current_label sigma) ->
+      Config (opaqueCall v) sigma ==>  Config (v_opa_l v lb) sigma  
   (* opaque call with return statement *)
   | ST_opaquecall_return2 : forall sigma sigma' s h lb s' lsf v,
       sigma = SIGMA s h->
@@ -408,35 +456,49 @@ Inductive step : tm -> Sigma -> tm -> Sigma -> Prop :=
       lb = (current_label sigma) ->
       sigma' = SIGMA s' h->
       value v ->
-      (opaqueCall (Return v)) / sigma ==> v_opa_l v lb / sigma'
+      Config (opaqueCall (Return v)) sigma ==> Config (v_opa_l v lb) sigma'
   | ST_opaquecall_return3 : forall sigma,
-      opaqueCall (Return null) / sigma ==> NPE / sigma
+      Config (opaqueCall (Return null)) sigma ==> Error_state
 
 
 (* assignment *)
   (* context rule *)
   | ST_assignment1 : forall sigma sigma' e e' id,
-       e / sigma ==>  e' / sigma' -> 
-       Assignment id e / sigma ==> Assignment id e' / sigma'
+       Config e sigma ==> Config e' sigma' -> 
+       Config (Assignment id e) sigma ==> Config (Assignment id e') sigma'
+  (* context rule error*)
+  | ST_assignment_ctx_error : forall sigma e id,
+      Config e sigma ==>  Error_state -> 
+     Config  (Assignment id e) sigma  ==>  Error_state
   (* assignment *)
   | ST_assignment2 : forall sigma sigma' id v s' s h,
        value v ->
        sigma = SIGMA s h ->
        s' = update_stack_top s id v->
        sigma' = SIGMA s' h ->
-       Assignment id v / sigma ==> Skip / sigma'
+       Config (Assignment id v) sigma ==> Config Skip sigma'
 
 (* Field Write *)
   (* context rule 1 *)
   | ST_fieldWrite1 : forall sigma sigma' f e1 e1' e2,
-       e1 / sigma ==>  e1' / sigma' -> 
-       FieldWrite e1 f e2 / sigma ==> FieldWrite e1' f e2/ sigma'
+       Config e1 sigma ==> Config e1' sigma' -> 
+       Config (FieldWrite e1 f e2) sigma ==> Config (FieldWrite e1' f e2) sigma'
+  (* context rule error 1 *)
+  | ST_fieldWrite_ctx_error1 : forall sigma f e1 e2,
+       Config e1 sigma ==> Error_state -> 
+       Config (FieldWrite e1 f e2) sigma ==> Error_state
   (* context rule 2 *)
   | ST_fieldWrite2 : forall sigma sigma' f v e2 e2',
        (forall t, value t -> t<> null -> e2 <> unlabelOpaque t) ->
        value v ->
-       e2 / sigma ==>  e2' / sigma' -> 
-       FieldWrite v f e2 / sigma ==> FieldWrite v f e2'/ sigma'
+       Config e2 sigma ==> Config e2' sigma' -> 
+       Config (FieldWrite v f e2) sigma ==> Config (FieldWrite v f e2') sigma'
+  (* context rule error 2 *)
+  | ST_fieldWrite_ctx_error2 : forall sigma f v e2,
+       (forall t, value t -> t<> null -> e2 <> unlabelOpaque t) ->
+       value v ->
+       Config e2 sigma ==> Error_state -> 
+       Config (FieldWrite v f e2) sigma ==> Error_state
   (* field write normal *)
   | ST_fieldWrite3 : forall sigma sigma' o s h h' f lb cls F F' v l',
       sigma = SIGMA s h ->
@@ -446,10 +508,10 @@ Inductive step : tm -> Sigma -> tm -> Sigma -> Prop :=
       h' = add_heap_obj h o (Heap_OBJ cls F' l') ->
       sigma' = SIGMA s h' ->
       value v->
-      (FieldWrite (ObjId o) f v) / sigma ==> Skip / sigma'
+      Config (FieldWrite (ObjId o) f v) sigma ==> Config Skip sigma'
   (* null pointer exception for field write *)
   | ST_fieldWriteException : forall sigma f v, 
-      (FieldWrite null f v) / sigma ==> NPE / sigma
+      Config (FieldWrite null f v) sigma ==> Error_state
   (* field write normal *)
   | ST_fieldWrite_opaque : forall sigma sigma' o s h h' f lo cls F F' v l' lb e2,
       e2 = unlabelOpaque (v_opa_l v lb) ->
@@ -459,16 +521,19 @@ Inductive step : tm -> Sigma -> tm -> Sigma -> Prop :=
       l' = join_label lo lb ->
       h' = add_heap_obj h o (Heap_OBJ cls F' l') ->
       sigma' = SIGMA s h' ->
-      (FieldWrite (ObjId o) f e2) / sigma ==> Skip / sigma'
+      Config (FieldWrite (ObjId o) f e2) sigma ==> Config Skip sigma'
   | ST_FieldWriteOpaqueDataException : forall sigma o f, 
-      FieldWrite (ObjId o) f (unlabelOpaque null) / sigma ==> NPE / sigma
-
+      Config (FieldWrite (ObjId o) f (unlabelOpaque null)) sigma ==> Error_state
 
 (* return statement *)
   (* context rule*)
   | ST_return1 : forall sigma sigma' e e',
-       e / sigma ==>  e' / sigma' -> 
-        Return e / sigma ==> Return e' / sigma'
+        Config e sigma ==> Config e' sigma' -> 
+        Config (Return e) sigma ==> Config (Return e') sigma'
+  (* context rule error*)
+  | ST_return_ctx_error : forall sigma e,
+        Config e sigma ==> Error_state -> 
+        Config (Return e) sigma ==> Error_state
   (* return val *)
   | ST_return2 : forall sigma sigma' v s s' s'' h lsf l', 
       value v ->
@@ -477,42 +542,44 @@ Inductive step : tm -> Sigma -> tm -> Sigma -> Prop :=
       l' = join_label (get_current_label s) (get_current_label s') ->
       s'' = update_current_label s' l' ->
       sigma' = SIGMA s'' h ->
-       Return v / sigma ==> v / sigma'
+      Config (Return v) sigma ==> Config v sigma'
 
 (* if statement *)
-  | ST_if_b1 : forall sigma s1 s2 v1 v2 s h lsf s' lb sf id1 id2, 
+  | ST_if_b1 : forall sigma s1 s2 s h lsf s' lb sf id1 id2, 
        sigma = SIGMA s h ->
        s = cons lsf s' ->
        lsf = Labeled_frame lb sf ->
-       Some v1 = sf(id1) ->
-       Some v2 = sf(id2) ->
-       v1 = v2 ->
-       If id1 id2 s1 s2 / sigma ==>  s1 / sigma
-  | ST_if_b2 : forall sigma s1 s2 v1 v2 s h lsf s' lb sf id1 id2, 
+       sf(id1) = sf(id2) ->
+       Config (If id1 id2 s1 s2) sigma ==> Config s1 sigma
+  | ST_if_b2 : forall sigma s1 s2 s h lsf s' lb sf id1 id2, 
        sigma = SIGMA s h ->
        s = cons lsf s' ->
        lsf = Labeled_frame lb sf ->
-       Some v1 = sf(id1) ->
-       Some v2 = sf(id2) ->
-       v1 <> v2 ->
-       If id1 id2 s1 s2 / sigma ==>  s2 / sigma
+       sf(id1) <> sf(id2) ->
+       Config (If id1 id2 s1 s2) sigma ==> Config s2 sigma
 (* sequence *)
    (* context rule *)
-  | ST_seq1 : forall sigma s1 s2 s1', 
-    Sequence s1 s2 / sigma ==> Sequence s1' s2 / sigma
+  | ST_seq1 : forall sigma s1 s2 s1' sigma', 
+    Config s1 sigma ==> Config s1' sigma' -> 
+    Config (Sequence s1 s2) sigma ==> Config (Sequence s1' s2) sigma'
+  (* context rule error *)   
+  | ST_seq_ctx_error : forall sigma s1 s2, 
+    Config s1 sigma ==> Error_state -> 
+    Config (Sequence s1 s2) sigma ==> Error_state
    (* sequence rule *)
   | ST_seq2 : forall sigma v s , 
     value v->
-    Sequence v s / sigma ==> s / sigma
+    Config (Sequence v s) sigma ==> Config s sigma
 
-where "c1 '/' st '==>' c1' '/' st'" := (step c1 st c1' st').
+where "c '==>' c'" := (reduction c c').
+
 
 Inductive ty : Type :=
   | classTy : cn -> ty 
   | LabelTy : ty
   | LabelelTy : ty -> ty
   | OpaqueLabeledTy : ty -> ty
-  | voidTy : ty.
+  | voidTy : ty. 
 
 Definition typing_context := id -> (option ty).
 Definition empty_context : typing_context := fun _ => None.
@@ -535,18 +602,19 @@ Inductive has_type : Class_table -> typing_context -> heap -> tm -> ty -> Prop :
       type_of_field fields_def f = Some cls' ->
       has_type CT Gamma h (FieldAccess e f) (classTy cls')
 (* method call *)
-  | T_MethodCall : forall Gamma e meth argu CT h T returnT cls_def body arg_id arguT para_T cls_a returnV,
+  | T_MethodCall : forall Gamma e meth argu CT h T returnT cls_def body arg_id arguT para_T cls_a,
       has_type CT Gamma h e (classTy T) ->
       has_type CT Gamma h argu arguT ->
       Some cls_def = CT(T) ->
-      find_method cls_def meth = Some (m_def returnT meth cls_a arg_id body (Return returnV))  ->
+      find_method cls_def meth = Some (m_def returnT meth cls_a arg_id (Return body))  ->
       arguT = para_T ->
-      has_type CT Gamma h (returnV) (classTy returnT) ->
+      has_type CT Gamma h (body) (classTy returnT) ->
       has_type CT Gamma h (MethodCall e meth argu) (classTy returnT)
 (* new exp *)
-  | T_NewExp : forall h Gamma cn CT cls_def,
-      Some cls_def = CT(cn) ->
-      has_type CT Gamma h (NewExp cn) (classTy cn)
+  | T_NewExp : forall h Gamma cls_name CT cls_def,
+      Some cls_def = CT(cls_name) ->
+      (exists field_defs method_defs, cls_def = class_def cls_name field_defs method_defs) ->
+      has_type CT Gamma h (NewExp cls_name) (classTy cls_name)
 (* label *)
   | T_label : forall h Gamma lb CT,
       has_type CT Gamma h (l lb) LabelTy
@@ -578,14 +646,14 @@ Inductive has_type : Class_table -> typing_context -> heap -> tm -> ty -> Prop :
   | T_assignment : forall h Gamma CT e T x,
       Gamma x = Some T ->
       has_type CT Gamma h e T ->
-      has_type CT Gamma h (Assignment x e) T
+      has_type CT Gamma h (Assignment x e) voidTy
 (* Field Write *)
   | T_FieldWrite : forall h Gamma x f cls_def CT clsT cls' e,
       has_type CT Gamma h x (classTy clsT) ->
       has_type CT Gamma h e (classTy cls') ->
       Some cls_def = CT(clsT) ->
       type_of_field (find_fields cls_def) f = Some cls' ->
-      has_type CT Gamma h (FieldWrite x f e) (classTy cls')
+      has_type CT Gamma h (FieldWrite x f e) voidTy
 (* if *)
   | T_if : forall Gamma h CT id1 id2 s1 s2 T T',
       Gamma id1 = Some (classTy T) ->
@@ -604,9 +672,10 @@ Inductive has_type : Class_table -> typing_context -> heap -> tm -> ty -> Prop :
       T <> voidTy ->
       has_type CT Gamma h (Return e) T
 (* ObjId *)
-  | T_ObjId : forall h Gamma CT o cls_name F lo cls_def,
+  | T_ObjId : forall h Gamma CT o cls_name cls_def,
       Some cls_def = CT(cls_name) ->
-      h(o) = Some (Heap_OBJ cls_def F lo) ->
+      (exists F lo, h(o) = Some (Heap_OBJ cls_def F lo)) ->
+      (exists field_defs method_defs, cls_def = (class_def cls_name field_defs method_defs)) ->
       has_type CT Gamma h (ObjId o) (classTy cls_name)
 (* NPE 
   | T_NPE : forall h Gamma CT T,
@@ -622,7 +691,6 @@ Inductive has_type : Class_table -> typing_context -> heap -> tm -> ty -> Prop :
       has_type CT Gamma h (l lb)  LabelTy ->
       has_type CT Gamma h v  T ->
       has_type CT Gamma h (v_opa_l v lb) (OpaqueLabeledTy T).
-
 
 Definition empty_heap : heap := fun _ => None.
 
@@ -640,20 +708,6 @@ Inductive wfe_fields : (list field) -> FieldMap -> Prop  :=
       fm(x) = Some v ->
       wfe_fields (cons h t) fm.
 
-
-(*
-Inductive wfe_heap : Class_table -> typing_context -> heap -> Prop :=
-  | empty_heap_wfe : forall ct ctx, wfe_heap ct ctx empty_heap
-  | heap_wfe : forall h h' cls_def F cn ct gamma fields newHo o lo,
-        (wfe_heap ct gamma h /\ h(o) = None)
-        -> newHo = Some (Heap_OBJ cls_def F lo)
-        -> Some cls_def  = ct cn
-        -> fields = (find_fields cls_def)
-        -> (forall f cls', type_of_field fields f = Some cls' -> exists v, F(f) = Some v )
-        -> h' = (fun x' => if beq_oid o x' then newHo else h x')
-        -> wfe_heap ct gamma h'.
-*)
-
 Inductive wfe_heap : Class_table -> typing_context -> heap -> Prop :=
   | empty_heap_wfe : forall ct ctx, wfe_heap ct ctx empty_heap
   | heap_wfe : forall h h' o cls_def F ct gamma cn ho lo method_defs field_defs,
@@ -663,7 +717,14 @@ Inductive wfe_heap : Class_table -> typing_context -> heap -> Prop :=
         h' = (fun x' => if beq_oid o x' then ho else (h x')) ->
         Some cls_def  = ct cn ->
         cls_def = class_def cn field_defs method_defs ->
-        (forall f cls', type_of_field field_defs f = Some cls' -> exists v, F(f) = Some v)->
+        (forall f cls', type_of_field field_defs f = Some cls' -> 
+                exists v, F(f) = Some v
+                 /\ (v= null  \/ 
+                          ( exists o' F' lx field_defs0 method_defs0, v = ObjId o' 
+                                  /\ h'(o') = Some (Heap_OBJ (class_def cls' field_defs0 method_defs0) F' lx)
+                                    /\ ct cls' = Some (class_def cls' field_defs0 method_defs0)
+                          ) )
+        )->
         (exists o', h' o' = None) ->
         wfe_heap ct gamma h'.
 
@@ -686,26 +747,11 @@ Lemma field_val_of_heap_obj : forall h o gamma CT cls_def F lo cls' fields,
 Proof with auto.
   intros. induction H. inversion H0. case_eq (beq_oid o0 o). intro.
   rewrite -> H5 in H0. rewrite -> H10 in H0. subst. inversion H0. subst.
-  apply H8 with (f:=f) (cls':=cls'). assumption.
+  destruct H8 with   (f:=f) (cls':=cls'). inversion H2. auto. destruct H1. 
+  exists x. auto. 
   intros. rewrite -> H5 in H0. rewrite -> H10 in H0. apply IHwfe_heap. assumption.
 
 Qed.
-
-(*
-Lemma field_val_of_heap_obj : forall cls_name h o gamma CT cls_def F lo cls' field_defs method_defs,
-  wfe_heap CT gamma h -> 
-  h(o) = Some (Heap_OBJ cls_def F lo) ->
-  cls_def =  (class_def cls_name field_defs method_defs) ->
-  CT cls_name = Some cls_def ->
-  (forall f, type_of_field field_defs f = Some cls' -> exists v, F(f) = Some v).
-Proof with auto.
-  intros. induction H. inversion H0. case_eq (beq_oid o0 o). intro.
-  rewrite -> H6 in H0. rewrite -> H11 in H0. subst. inversion H0. subst.
-  apply H9 with (f:=f) (cls':=cls'). assumption.
-  intros. rewrite -> H6 in H0. rewrite -> H11 in H0. apply IHwfe_heap. assumption. assumption.
-Qed.
-*)
-
 
 Lemma empty_heap_empty :
   ~ exists x cls F lo, empty_heap x = Some (Heap_OBJ cls F lo).
@@ -737,12 +783,19 @@ Fixpoint variable_exists (s : stack) (x : id) :=
                                         end
   end.
 
-Inductive wfe_stack_frame : heap -> labeled_stack_frame -> Prop :=
-  | stack_frame_wfe : forall h lsf sf o lb,
+Inductive wfe_stack_frame : Class_table -> typing_context -> heap -> labeled_stack_frame -> Prop :=
+  | stack_frame_wfe : forall h lsf sf lb ct gamma,
         lsf = Labeled_frame lb sf ->
-        (forall x v, sf x = Some v ->
-        v = null \/ ( v = ObjId o /\ (exists F lo cls_def, h(o) = Some (Heap_OBJ cls_def F lo)) )) ->
-        wfe_stack_frame h lsf. 
+        (forall cls_name x, gamma x = Some (classTy cls_name) 
+        -> exists v, sf x = Some v   
+              /\ ( v = null \/ 
+                 ( exists o, v = ObjId o 
+(*                              /\ gamma x = Some (classTy cls_name)*)
+                              /\ (exists F lo field_defs method_defs , h(o) = Some (Heap_OBJ (class_def cls_name field_defs method_defs) F lo)
+                                      /\ (ct cls_name = Some (class_def cls_name field_defs method_defs))
+                                   ) 
+                  )    ) ) ->
+        wfe_stack_frame ct gamma h lsf. 
 
 
 Inductive wfe_stack : Class_table -> typing_context -> heap -> stack -> Prop :=
@@ -751,17 +804,22 @@ Inductive wfe_stack : Class_table -> typing_context -> heap -> stack -> Prop :=
         h = empty_heap ->
         gamma = empty_context -> 
         wfe_stack ct gamma h (cons main_labeled_stack_frame nil)
-  | stack_wfe : forall s ct h gamma x T s' lb sf cls_def gamma' v v', 
+  | stack_wfe : forall s ct gamma x s' lb sf gamma' v' h, 
         s = cons (Labeled_frame lb sf) s'->
         wfe_stack ct gamma h s' ->
         wfe_heap ct gamma h ->
-        wfe_stack_frame h ((Labeled_frame lb sf)) ->
-        gamma x = None ->
-        variable_exists s' x = false ->
-        sf x = Some v ->
+        gamma x = None ->        
         sf (Id "this") = Some v' ->
-        gamma'= (fun x' => if beq_id x x' then (Some (classTy T)) else (gamma x)) ->
-        ct T = Some cls_def -> 
+(*        variable_exists s' x = false ->
+        sf x = Some v ->
+        gamma'= (fun x' => if beq_id x x' then (Some T) else (gamma x)) ->
+        (exists o, v = ObjId o -> exists cls_name F lo field_defs method_defs, 
+                      T = classTy cls_name /\                
+                      h o = Some (Heap_OBJ (class_def cls_name field_defs method_defs) F lo) /\
+                      ct cls_name = Some (class_def cls_name field_defs method_defs)
+        ) -> 
+*)
+        wfe_stack_frame ct gamma' h (Labeled_frame lb sf) ->
         wfe_stack ct gamma' h s.
 
 Lemma beq_equal : forall x x', beq_id x x' = true -> x' = x.
@@ -773,18 +831,45 @@ Proof.
   - intro. intro. rewrite -> H0 in H. inversion H. 
 Qed.
 
+Theorem beq_nat_true: forall n m,
+  beq_nat n m = true -> n = m.
+Proof.
+  intros n. induction n.
+    intros. destruct m. 
+      reflexivity.  inversion H.
+    intros. destruct m. 
+      inversion H. simpl in H. apply f_equal. apply IHn in H. apply H.
+Qed. 
+
+Lemma beq_oid_same : forall o, beq_oid o o = true. 
+Proof with auto. 
+  intro o. unfold beq_oid. destruct o. induction n. reflexivity.
+  simpl. auto. 
+Qed. 
+
+Lemma beq_oid_equal : forall x x', beq_oid x x' = true -> x = x'.
+Proof.
+   intros. unfold beq_oid in H.
+   destruct x. destruct x'. f_equal. 
+   case_eq (n =? n0). intro. 
+   apply beq_nat_true with (n:=n) (m:=n0). auto. 
+
+   intro. rewrite H0 in H. inversion H.
+Qed.
+
 Lemma Typed_variable : forall sigma s h ct gamma x T sf s' lb,
   sigma = SIGMA s h ->
   wfe_stack ct gamma h s ->
-   gamma x = Some T -> 
+   gamma x = Some (classTy T) -> 
    s = cons (Labeled_frame lb sf) s' -> 
    exists v, sf x = Some v.
 Proof with eauto.
   intros. inversion H0.
   + subst. inversion H1. 
-  + subst. case_eq (beq_id x0 x). intros. rewrite -> H in H1. inversion H1. subst. - exists v. rewrite <- H9. 
-        inversion H3. subst. f_equal. apply beq_equal. assumption.
- - intros. rewrite -> H in H1. rewrite -> H7 in H1. inversion H1.  
+  + subst. inversion H3. 
+        inversion H8. 
+        destruct H11 with T x. auto. 
+        destruct H16. inversion H. exists x1. auto. 
 Qed.
 
 Inductive wfe : Class_table -> typing_context -> Sigma -> Prop :=
@@ -807,8 +892,6 @@ Proof with eauto.
   intros. rewrite -> H. auto.
 Qed. 
 
-Check f_equal.
-
 Lemma wfe_oid : forall o ct gamma s h sigma cls_def cn, 
   sigma = SIGMA s h ->
   wfe_stack ct gamma h s ->
@@ -816,8 +899,8 @@ Lemma wfe_oid : forall o ct gamma s h sigma cls_def cn,
     -> exists fieldsMap lb, h(o) = Some (Heap_OBJ cls_def fieldsMap lb).
 Proof with auto. 
   intros. inversion H0. 
-    - inversion H1. subst. inversion H16.
-    - inversion H1. subst. exists F. rewrite <- H22 in H2. inversion H2. exists lo. rewrite -> H3 in H23. assumption.  
+    - inversion H1. subst. inversion H16. destruct H as [lo]. inversion H.
+    - inversion H1. rewrite H2 in H15. inversion H15. rewrite <- H22.  auto. 
 Qed.
 
 Definition val_option_type (input : option tm) : tm :=
@@ -840,7 +923,6 @@ right. intro.  intros contra. inversion contra.
 right. intro.  intros contra. inversion contra.
 
 left. exists t. auto. 
-right. intro.  intros contra. inversion contra.
 right. intro.  intros contra. inversion contra.
 right. intro.  intros contra. inversion contra.
 right. intro.  intros contra. inversion contra.
@@ -876,7 +958,6 @@ left. exists t.  auto.
 right. intro.  intros contra. inversion contra.
 right. intro.  intros contra. inversion contra.
 right. intro.  intros contra. inversion contra.
-right. intro.  intros contra. inversion contra.
 Qed.
 
 
@@ -886,11 +967,10 @@ Proof with auto.
   intros. inversion H1. exists main_labeled_stack_frame. exists nil. auto. 
   exists (Labeled_frame lb sf). exists s'. auto. 
 Qed.
- 
 
 Theorem progress : forall t T sigma gamma CT s h, 
   sigma = SIGMA s h ->  wfe_heap CT gamma h -> wfe_stack CT gamma h s -> 
-  has_type CT gamma h t T -> value t \/ exists t' sigma', t / sigma ==> t' / sigma'.
+  has_type CT gamma h t T -> value t \/ (exists config', Config t sigma ==> config').
 Proof with auto.
   intros t T sigma gamma CT s h.
   intros. 
@@ -898,15 +978,17 @@ Proof with auto.
   induction H2. 
 (* TVar *)
 - right. 
-      inversion H1. + subst. inversion H2.
-                    + subst. exists v. exists (SIGMA (Labeled_frame lb sf :: s') h).
+      inversion H1. 
+          + subst. inversion H2.
+          + subst. inversion H8.  destruct H3 with T x. auto. 
+             destruct H13. exists (Config x1 (SIGMA (Labeled_frame lb sf :: s') h)).
+              
 
       apply ST_var with 
-      (id:=x) (lb:=lb) (sf:=sf) (lsf:=Labeled_frame lb sf) (v:=v) 
+      (id:=x) (lb:=lb) (sf:=sf) (lsf:=Labeled_frame lb sf) (v:=x1) 
       (sigma:=(SIGMA (Labeled_frame lb sf :: s') h)) (s':=s') (s:=(Labeled_frame lb sf :: s')) (h:=h).
-      auto. auto. auto. 
-      case_eq (beq_id x0 x). intro. apply beq_equal with (x:=x0) (x':=x) in H. subst. auto.
-      intro. rewrite -> H in H2. rewrite -> H7 in H2. inversion H2.   
+      auto. auto. auto. inversion H. intuition. 
+
 (* null *)
 -  left. apply v_null.
 (* field access *)
@@ -928,15 +1010,15 @@ Proof with auto.
       destruct H9 as [v].
       remember (join_label lb (current_label sigma)) as l'.
       remember (update_current_label s l') as s'.
-      remember (SIGMA s' (get_heap sigma)) as sigma'.
-            exists v. exists sigma'. apply ST_fieldRead2 with 
+      remember (SIGMA s' h) as sigma'.
+            exists (Config v sigma'). apply ST_fieldRead2 with 
             (sigma:=sigma) (sigma':=sigma') (o:=o) (s:=s) (h:=h) (fname:=f) (lb:=lb) 
             (cls:=cls_def) (fields:=F) (v:=v) (l':=l') (s':=s'). 
             auto. auto. auto.            auto. auto. auto. 
     (* skip *)
     rewrite <- H7 in H2. inversion H2. 
     (* call field access on null point object *)
-    exists NPE. exists sigma. apply ST_fieldReadException.
+    exists Error_state. apply ST_fieldReadException.
     (* label is primitive: calling field access is not valid *)
     rewrite <- H7 in H2. inversion H2.
    
@@ -947,9 +1029,12 @@ Proof with auto.
     {rewrite <- H7  in H2. inversion H2. }
 
      (* context rule *)
-    + { destruct H6 as [e']. destruct H6 as [sigma'].
-    exists (FieldAccess e' f). exists sigma'.
-    apply ST_fieldRead1 with (sigma:=sigma) (sigma':=sigma') (e:=e) (e':=e') (f:=f). assumption. }
+    + destruct H6. destruct x. 
+    exists (Config (FieldAccess t f) s0).
+    apply ST_fieldRead1 with (sigma:=sigma) (sigma':=s0) (e:=e) (e':=t) (f:=f). assumption.
+
+    exists Error_state. apply ST_fieldRead3. auto. 
+    
 
 (* method call *)
 - right.
@@ -963,25 +1048,25 @@ Proof with auto.
             remember (Labeled_frame l sf) as lsf. 
             remember (cons lsf s) as s'.
             remember (SIGMA s' (get_heap sigma)) as sigma'.
-            exists (Sequence body (Return returnV)) . exists sigma'.
+            exists (Config ((Return body)) sigma').
+            destruct H13 as [F]. destruct H as [lo].
             apply ST_MethodCall3 with (sigma:=sigma) (sigma':=sigma') (o:=o) (s:=s) (h:=h) (cls:=cls_def) (fields:=F) 
                                        (v:=argu) (lx:=lo) (l:=l) 
                                        (theta:=lsf) (s':=s') (sf:=sf) (lsf:=lsf) (arg_id:=arg_id) 
-                                        (cls_a:=cls_a) (body:=body) (meth:=meth) (returnT:=returnT) (return_v:=returnV); auto.
-            rewrite <- H12 in H2. inversion H2. rewrite <- H13; auto. 
+                                        (cls_a:=cls_a) (body:=body) (meth:=meth) (returnT:=returnT) ;auto.
+            rewrite <- H9 in H2. inversion H2.  auto. 
           (* case analysis for argument, if the argument is not a value *)
-            subst. 
-                destruct H14 as [t']. destruct H as [sigma'].
+            subst.
+                destruct H15 as [config']. destruct config' as [t' | sigma']. 
                 pose proof (excluded_middle_opaqueLabel argu).
                 destruct H4.
                   (* case for argu = unlabelOpaque t *)
                   destruct H4 as [t]. 
                   rewrite -> H4 in H. inversion H. subst. 
-                  exists (MethodCall (ObjId o) meth (unlabelOpaque e')).
-                  exists (sigma').
-                  apply ST_MethodCall2 with (sigma:=(SIGMA s h)) (sigma':=sigma') 
+                  exists (Config (MethodCall (ObjId o) meth (unlabelOpaque e')) s0).
+                  apply ST_MethodCall2 with (sigma:=(SIGMA s h)) (sigma':=s0) 
                                             (v:=(ObjId o)) (e:=unlabelOpaque t) (e':=unlabelOpaque e') (id:=meth).
-                  intros. subst. intro contra. inversion contra. rewrite -> H9 in H. inversion H4.
+                  intros. subst. intro contra. inversion contra. rewrite -> H10 in H. inversion H4.
                       rewrite <- H8 in H; subst; inversion H7. auto.  subst. inversion H7.  subst.
                       inversion H7. subst. inversion H7. subst. inversion H7. subst. inversion H7.
                       assumption. apply v_oid. 
@@ -992,61 +1077,79 @@ Proof with auto.
                       remember (Labeled_frame l' sf) as lsf. 
                       remember (cons lsf s) as s'.
                       remember (SIGMA s' (get_heap sigma)) as sigma''.
-                      exists (Sequence body (Return returnV)). exists sigma''. 
+                      exists (Config (Return body) sigma'').  
+                      destruct H13 as [F]. destruct H4 as [lo].
                       apply ST_MethodCall_unlableOpaque with (sigma:=sigma) (sigma':=sigma'') (o:=o) (s:=s) (h:=h) 
                                             (cls:=cls_def0) (fields:=F) (v:=t') (lx:=lo) (l':=l') (lb:=lb) (s':=s')
                                            (sf:=sf) (lsf:=lsf) (arg_id:=arg_id) (cls_a:=cls_a) (body:=body) 
-                                           (meth:=meth) (returnT:=returnT) (return_v:=returnV).
+                                           (meth:=meth) (returnT:=returnT) .
                       auto. auto. auto. auto. auto. auto. subst. 
-                      rewrite <- H12 in H2. inversion H2. rewrite <- H6. rewrite -> H3; auto. 
+                      rewrite <- H9 in H2. inversion H2. rewrite <- H7. auto. 
                       auto.
-                  (*exception case *)
+                  (*exception case
                   subst. exists NPE. exists (SIGMA s h).
-                  apply ST_MethodCallOpaqueDataException with (sigma:=(SIGMA s h)) (o:=o).  
+                  apply ST_MethodCallOpaqueDataException with (sigma:=(SIGMA s h)) (o:=o).   *)
 
                   (* case for argu <> unlabelOpaque t *)
-                  exists (MethodCall (ObjId o) meth t'). exists sigma'. 
-                  apply ST_MethodCall2 with (sigma:=(SIGMA s h)) (sigma':=sigma') (v:=((ObjId o))) 
+                  exists (Config (MethodCall (ObjId o) meth t') s0). 
+                  apply ST_MethodCall2 with (sigma:=(SIGMA s h)) (sigma':=s0) (v:=((ObjId o))) 
                                             (e:=argu) (e':=t') (id:=meth).
                   intro. intro. intro. 
 
                   assert (argu <> unlabelOpaque t).  apply (H4 t). apply (H4 t). auto. apply v_oid.
-                    
-                  rewrite <- H6 in H2_. inversion H2_.
-      
-                  (* case for argu <> unlabelOpaque t exception *)
-                  subst. exists NPE. exists (SIGMA s h). 
-              apply ST_MethodCallException with (sigma:=(SIGMA s h)) (v:=argu) (meth:=meth).
+                   
+                  exists Error_state. 
+                   apply ST_MethodCall5 with (sigma:=(SIGMA s h)) (v:=(ObjId o)) (e:=argu) (id:=meth).
+                  intros. intro contra. rewrite contra in H. inversion H. inversion H4. 
+                  rewrite <- H11 in H8. inversion H8.   rewrite <- H11 in H8. inversion H8.
+                  rewrite <- H11 in H8. inversion H8.   rewrite <- H11 in H8. inversion H8.
+                  rewrite <- H11 in H8. inversion H8.   rewrite <- H11 in H8. inversion H8.
+                  rewrite <- H8 in H6. auto. auto. auto. subst. inversion H2_. 
 
-                  subst. inversion H2_.
+                   exists Error_state. 
+                  apply ST_MethodCallException with (sigma:=sigma) (v:=argu) (meth:=meth). 
+
+                  rewrite <- H6 in H2_. inversion H2_. 
                 rewrite <- H6 in H2_. inversion H2_.                 rewrite <- H6 in H2_. inversion H2_. 
-      +  destruct H5 as [t']. destruct H5 as [sigma']. exists (MethodCall t' meth argu). exists (sigma').   
-                  apply ST_MethodCall1 with (sigma:=sigma) (sigma':=sigma') (e2:=argu) (e:=e) (e':=t') (id:=meth). apply H5.
+      +  destruct H5 as [config']. destruct config'. 
+
+            exists (Config (MethodCall t meth argu) (s0)).
+                  apply ST_MethodCall1 with (sigma:=sigma) (sigma':=s0) (e2:=argu) (e:=e) (e':=t) (id:=meth). apply H5.
+
+            exists Error_state. apply ST_MethodCall4 with (sigma:=sigma) (e:=e) (e2:=argu) (id:=meth). auto. 
 
 (* new expression *)
 - right. inversion H0. 
     assert (exists o, empty_heap o = None). 
       unfold empty_heap. auto. exists (OID 0). auto. 
-      destruct H6 as [o]. 
+      destruct H7 as [o]. 
 
       remember (init_field_map (find_fields cls_def) empty_field_map) as F.
       remember (current_label sigma) as lb. 
       remember  (add_heap_obj h o (Heap_OBJ cls_def F lb)) as h'.
       remember (SIGMA s h') as sigma'.
-      exists (ObjId o). exists sigma'. apply ST_NewExp with (sigma:=sigma) (sigma':=sigma') (F:=F) (o:=o) (h:=h) (cls:=cls_def)
-                                                                                (h':=h') (s:=s) (lb:=lb) (cn:=cn0).
-      subst; auto. rewrite <- H5.  auto.  auto. auto. auto.  auto. 
+      exists (Config (ObjId o) sigma').
+       
+      destruct H3 as [field_defs]. destruct H3 as [method_defs].
+      apply ST_NewExp with (sigma:=sigma) (sigma':=sigma') (F:=F) (o:=o) (h:=h) (cls:=cls_def)
+                  (h':=h') (s:=s) (lb:=lb) (cls_name:=cls_name) 
+                  (field_defs:= field_defs) (method_defs:=method_defs).
+
+      subst; auto. rewrite <- H6.  auto.  auto. auto. auto.  auto. auto.  
       
       remember (current_label sigma) as lb. 
-      destruct H10. 
+      destruct H11.
       remember (init_field_map (find_fields cls_def) empty_field_map) as F'.
       remember (add_heap_obj h x (Heap_OBJ cls_def F' lb)) as h''.
       remember (SIGMA s h'') as sigma''.
-      exists (ObjId x). exists sigma''. 
+      exists (Config (ObjId x) sigma''). 
+      destruct H3 as [field_defs']. destruct H3 as [method_defs'].
 
-      apply ST_NewExp with (sigma:=sigma) (sigma':=sigma'') (F:=F') (o:=x) (h:=h) (cls:=cls_def)
-                                                                                (h':=h'') (s:=s) (lb:=lb) (cn:=cn0).
-      auto. auto.  auto.  auto. auto. auto. 
+      apply ST_NewExp with (sigma:=sigma) (sigma':=sigma'') 
+                                          (F:=F') (o:=x) (h:=h) (cls:=cls_def)
+                                          (h':=h'') (s:=s) (lb:=lb) (cls_name:=cls_name)
+                                          (field_defs:=field_defs') (method_defs:=method_defs').
+      auto. auto.  auto.  auto. auto. auto.  auto.
 
 (* label *)
 - left. apply  v_label.
@@ -1057,7 +1160,7 @@ Proof with auto.
             destruct IHhas_type1. auto. auto. auto. 
             
             (* subgoal #1 *)
-           exists  (v_l e lb). exists sigma.
+           exists (Config (v_l e lb)sigma).
                 apply ST_LabelData2 with (sigma:=sigma) (lb:=lb) (v:=e). subst. auto.  auto.
 
             (*
@@ -1074,45 +1177,48 @@ Proof with auto.
             *)
 
             (* subgoal #2 *)  
-                destruct H3 as [t']. destruct H3 as [sigma']. inversion H3. 
+                destruct H3 as [config']. inversion H3.  
 
             (* subgoal #3 *)
-            destruct IHhas_type1. auto. auto. auto. 
-                   (* subgoal #4 *)
-                    destruct H2 as [t']. destruct H2 as [sigma'].
-                    exists (labelData t' lb). exists sigma'. 
-                    apply ST_LabelData1 with (sigma:=sigma) (sigma':=sigma') (e:=e) (e':=t') (lb:=lb).
-                    auto. 
-                   (* subgoal #5 *)
-                    destruct H2 as [t']. destruct H2 as [sigma']. 
-                    exists (labelData t' lb). exists sigma'.
-                    apply ST_LabelData1 with (sigma:=sigma) (sigma':=sigma') (e:=e) (e':=t') (lb:=lb).
+                destruct H2 as [config']. destruct config'. 
+                    exists (Config (labelData t lb) s0).
+                    apply ST_LabelData1 with (sigma:=sigma) (sigma':=s0) (e:=e) (e':=t) (lb:=lb).
                     auto.
 
+           (* subgoal #4*)
+               exists Error_state. 
+                  apply ST_LabelDataError with (e:=e) (sigma:=sigma) (lb:=lb). auto. 
+
 (* unlabel : *)
-- right. 
+- right.
+ 
             destruct IHhas_type. auto. auto. auto. 
              (* subgoal #1 *)
-                + inversion H3. rewrite <- H4 in H2. inversion H2. 
+                + inversion H3. 
+                     rewrite <- H4 in H2. inversion H2. 
                      rewrite <- H4 in H2.  inversion H2. 
-                    exists NPE. exists sigma.  apply ST_unlabelDataException with (sigma:=sigma).
-                    rewrite <- H4 in H2.  inversion H2. 
+                    exists Error_state.  apply ST_unlabelDataException with (sigma:=sigma).
+                    rewrite <- H4 in H2.  inversion H2.
 
              (* subgoal #2 *)
                 remember ( join_label lb (current_label sigma)) as l'.
                 remember (update_current_label s l') as s'.
                 remember (SIGMA s' (get_heap sigma)) as sigma'.
-                exists v. exists sigma'. 
+                exists (Config v sigma'). 
                 apply ST_unlabel2 with (sigma:=sigma) (s':=s') (sigma':=sigma') (l':=l') (s:=s) (h:=h) (lb:=lb) (v:=v). 
                 auto. auto. auto. auto. auto.
 
             (* subgoal #3 *)
                 rewrite <- H4 in H2.  inversion H2. 
 
-             (* subgoal #4 *)
-                + destruct H3 as [t']. destruct H3 as [sigma']. 
-                    exists  (unlabel t'). exists sigma'. apply ST_unlabel1 with (sigma:=sigma) (sigma':=sigma') (e:=e) (e':=t'). auto. 
-          
+              + destruct H3 as [config']. 
+                 destruct config'. 
+                 exists (Config (unlabel t) s0). 
+                 apply ST_unlabel1 with (sigma:=sigma) (sigma':=s0) (e:=e) (e':=t). auto. 
+                 exists Error_state. apply ST_unlabelContextError with (sigma:=sigma) (e:=e). auto. 
+  
+
+
 (* label Of *)
 (* same issue as above, we may need to add (v_l v lb) as a value*)
 - right. 
@@ -1120,15 +1226,18 @@ Proof with auto.
             (* subgoal #1 *)
                 + inversion H3. rewrite <- H4 in H2. inversion H2. 
                     rewrite <- H4 in H2. inversion H2. 
-                    exists NPE. exists sigma.  apply ST_labelOfDataException with (sigma:=sigma).
+                    exists Error_state.  apply ST_labelOfDataException with (sigma:=sigma).
                     rewrite <- H4 in H2.  inversion H2.
                     
-                   exists (l lb). exists (sigma). apply ST_labelof2 with (v:=v) (lb:=lb).
+                   exists (Config (l lb) (sigma)). apply ST_labelof2 with (v:=v) (lb:=lb).
 
                     rewrite <- H4 in H2. inversion H2. 
              (* subgoal #2 *)
-                + destruct H3 as [t']. destruct H3 as [sigma']. 
-                    exists  (labelOf t'). exists sigma'. apply ST_labelof1 with (sigma:=sigma) (sigma':=sigma') (e:=e) (e':=t'). auto. 
+                + destruct H3 as [config']. destruct config'. 
+                    exists (Config (labelOf t) s0). apply ST_labelof1 with (sigma:=sigma) (sigma':=s0) (e:=e) (e':=t). auto.
+    
+             (*error state *)
+                 exists Error_state. apply ST_labelofCtxError with (e:=e) (sigma:=sigma). auto. 
 
 (* unlabel opaque *)
 - right. 
@@ -1136,7 +1245,7 @@ Proof with auto.
             (* subgoal #1 *)
                 + inversion H3. rewrite <- H4 in H2. inversion H2. 
                     rewrite <- H4 in H2. inversion H2. 
-                    exists NPE. exists sigma.  apply ST_unlabel_opaqueDataException with (sigma:=sigma).
+                    exists Error_state.  apply ST_unlabel_opaqueDataException with (sigma:=sigma).
                     rewrite <- H4 in H2.  inversion H2.
               
                      rewrite <- H4 in H2. inversion H2. 
@@ -1144,154 +1253,57 @@ Proof with auto.
                 remember ( join_label lb (current_label sigma)) as l'.
                 remember (update_current_label s l') as s'.
                 remember (SIGMA s' (get_heap sigma)) as sigma'.
-                exists v. exists sigma'. 
+                exists (Config v sigma'). 
                 apply ST_unlabel_opaque2 with (sigma:=sigma) (s':=s') (sigma':=sigma') (l':=l') (s:=s) (h:=h) (lb:=lb) (v:=v). 
                 auto. auto. auto. auto. 
 
              (* subgoal #2 *)
-                + destruct H3 as [t']. destruct H3 as [sigma']. 
-                    exists  (unlabelOpaque t'). exists sigma'. apply ST_unlabel_opaque1 with (sigma:=sigma) (sigma':=sigma') (e:=e) (e':=t'). auto. 
+                + destruct H3 as [config']. destruct config'. 
+                    exists (Config (unlabelOpaque t) s0). apply ST_unlabel_opaque1 with (sigma:=sigma) (sigma':=s0) (e:=e) (e':=t). auto.
+
+                exists Error_state. apply ST_unlabel_opaque_ctx_error with (sigma:=sigma) (e:=e).  auto. 
 
 (* opaque call *)
-- right.  destruct IHhas_type. auto. auto. auto.    
-            exists e. exists sigma. apply ST_opaquecall_val2 with (v:=e) (sigma:=sigma). auto.
+- right.  destruct IHhas_type. auto. auto. auto.
+            (* opaquecall won't be applied on values  *)
 
-            subst. destruct H3 as [t']. destruct H as [sigma'].
+            remember (current_label sigma) as lb. 
+            exists (Config (v_opa_l e lb)  sigma). 
+            apply ST_opaquecall_val2 with (v:=e) (sigma:=sigma) (lb:=lb). auto. auto. 
+
+            subst. destruct H3 as [config'].
                 pose proof (excluded_middle_returnT e).
                 destruct H3.
-                  (* case for argu = return t *)
+                  (* case for e = return t *)
                   destruct H3 as [t].
-                  destruct t.
                   rewrite -> H3 in H. 
                   inversion H.  subst. 
-                  exists (opaqueCall(Return e')). exists sigma'.
-                  apply ST_opaquecall_return1 with (sigma:=(SIGMA s h)) (sigma':=sigma') (e:= (Tvar i)) (e':= e').
+                  exists (Config (opaqueCall(Return e')) sigma').
+                  apply ST_opaquecall_return1 with (sigma:=(SIGMA s h)) (sigma':=sigma') (e:= t) (e':=e').
+                  auto.
+
+                  exists Error_state. rewrite H3.  apply ST_opaquecall_return_error with (sigma:=(SIGMA s h)) (e:=t).
                   auto. 
 
-                  rewrite <- H11 in H. inversion H5. 
+                  destruct config'.
+                  remember  (current_label sigma) as lb. 
+                  exists (Config (v_opa_l t lb) (SIGMA s' h)).
+                  rewrite H3. 
+                  apply ST_opaquecall_return2 with (sigma:=(SIGMA s h) ) (sigma':=(SIGMA s' h)) (s:=s) (h:=h) 
+                                            (lb:=lb) (s':=s') (lsf:=lsf) (v:=t).
+                  auto. inversion H7.  auto. rewrite <- H5.  auto. auto. auto.
 
-                  (* subgoal *)
-                  subst. exists NPE. exists (SIGMA s h). 
-                  apply ST_opaquecall_return3 with (sigma:=(SIGMA s h)).
-                  (* subgoal field access*)
-                  subst. 
-                  exists (opaqueCall(t') ). exists sigma'.
-                  apply ST_opaquecall1 with (sigma:=(SIGMA s h)) (sigma':=sigma') (e:= Return (FieldAccess t i) ) (e':= t').
-                  intros. intro contra. inversion contra. rewrite <- H5 in H3.  inversion H3.         auto.
-                  (* method call *)
-                  subst. 
-                  exists (opaqueCall(t') ). exists sigma'.
-                  apply ST_opaquecall1 with (sigma:=(SIGMA s h)) (sigma':=sigma') (e:= Return (MethodCall t1 i t2) ) (e':= t').
-                  intros. intro contra. inversion contra. rewrite <- H5 in H3.  inversion H3.         auto.
-                  (* new expression *)
-                  subst. 
-                  exists (opaqueCall(t') ). exists sigma'.
-                  apply ST_opaquecall1 with (sigma:=(SIGMA s h)) (sigma':=sigma') (e:= Return (NewExp c) ) (e':= t').
-                  intros. intro contra. inversion contra. rewrite <- H5 in H3.  inversion H3.         auto.
-                  (* return label : when e <> return v*)
-                  subst. 
-                  remember (SIGMA s h)  as sigma. 
-                  assert (exists lsf s', s = cons lsf s'). apply stack_not_nil with (sigma:=(SIGMA s h)) (s:=s) (h:=h) (gamma:=Gamma) (CT:=CT).
-                  auto. auto. auto. 
-                  destruct H3 as [lsf].  destruct H3 as [s'].
-                  remember (current_label sigma) as lb. 
-                  remember (SIGMA s' h) as sigma''.
-                  exists (v_opa_l (l l0) lb). exists sigma''. 
-                  apply ST_opaquecall_return2 with (sigma:=sigma) (sigma':=sigma'') (s:=s) (h:=h) (lb:=lb) (s':=s') (lsf:=lsf) (v:=(l l0)). 
-                  auto. auto. auto. auto. apply v_label. 
-                  
-                  
-                  subst. 
-                  exists (opaqueCall(t') ). exists sigma'.
-                  apply ST_opaquecall1 with (sigma:=(SIGMA s h)) (sigma':=sigma') (e:= Return (labelData t l0) ) (e':= t').
-                  intros. intro contra. inversion contra. rewrite <- H5 in H3.  inversion H3.         auto.
+                  inversion H11. 
 
-                  subst. 
-                  exists (opaqueCall(t') ). exists sigma'.
-                  apply ST_opaquecall1 with (sigma:=(SIGMA s h)) (sigma':=sigma') (e:= Return (unlabel t) ) (e':= t').
-                  intros. intro contra. inversion contra. rewrite <- H5 in H3.  inversion H3.         auto.
+                    (* case for e <> return t *)
 
-                  subst. 
-                  exists (opaqueCall(t') ). exists sigma'.
-                  apply ST_opaquecall1 with (sigma:=(SIGMA s h)) (sigma':=sigma') (e:= Return (labelOf t) ) (e':= t').
-                  intros. intro contra. inversion contra. rewrite <- H5 in H3.  inversion H3.         auto.
+                  destruct config'. 
+                  exists (Config (opaqueCall t) s0). 
+                  apply ST_opaquecall1 with  (sigma:=(SIGMA s h) ) (sigma':=(s0)) (e:=e) (e':=t). 
 
-                  subst. 
-                  exists (opaqueCall(t') ). exists sigma'.
-                  apply ST_opaquecall1 with (sigma:=(SIGMA s h)) (sigma':=sigma') (e:= Return (unlabelOpaque t) ) (e':= t').
-                  intros. intro contra. inversion contra. rewrite <- H5 in H3.  inversion H3.         auto.
+                  intros. apply H3. auto. 
 
-                  subst. 
-                  exists (opaqueCall(t') ). exists sigma'.
-                  apply ST_opaquecall1 with (sigma:=(SIGMA s h)) (sigma':=sigma') (e:= Return (opaqueCall t) ) (e':= t').
-                  intros. intro contra. inversion contra. rewrite <- H5 in H3.  inversion H3.         auto.
-
-                   rewrite -> H3 in H2. inversion H2. inversion H5. rewrite -> H15 in H9. intuition.
-
-                  subst. 
-                  exists (opaqueCall(t') ). exists sigma'.
-                  apply ST_opaquecall1 with (sigma:=(SIGMA s h)) (sigma':=sigma') (e:= Return (Assignment i t) ) (e':= t').
-                  intros. intro contra. inversion contra. rewrite <- H5 in H3.  inversion H3.         auto.
-
-                  subst. 
-                  exists (opaqueCall(t') ). exists sigma'.
-                  apply ST_opaquecall1 with (sigma:=(SIGMA s h)) (sigma':=sigma') (e:= Return (FieldWrite t1 i t2)) (e':= t').
-                  intros. intro contra. inversion contra. rewrite <- H5 in H3.  inversion H3.         auto.
-
-                  subst. 
-                  exists (opaqueCall(t') ). exists sigma'.
-                  apply ST_opaquecall1 with (sigma:=(SIGMA s h)) (sigma':=sigma') (e:= Return (If i i0 t1 t2)) (e':= t').
-                  intros. intro contra. inversion contra. rewrite <- H5 in H3.  inversion H3.         auto.
-
-                  subst. 
-                  exists (opaqueCall(t') ). exists sigma'.
-                  apply ST_opaquecall1 with (sigma:=(SIGMA s h)) (sigma':=sigma') (e:= Return (Sequence t1 t2)) (e':= t').
-                  intros. intro contra. inversion contra. rewrite <- H5 in H3.  inversion H3.         auto.
-
-                  subst. 
-                  exists (opaqueCall(t') ). exists sigma'.
-                  apply ST_opaquecall1 with (sigma:=(SIGMA s h)) (sigma':=sigma') (e:= Return (Return t)) (e':= t').
-                  intros. intro contra. inversion contra. rewrite <- H5 in H3.  inversion H3.         auto.
-
-                  subst. 
-                  remember (SIGMA s h)  as sigma. 
-                  assert (exists lsf s', s = cons lsf s'). apply stack_not_nil with (sigma:=(SIGMA s h)) (s:=s) (h:=h) (gamma:=Gamma) (CT:=CT).
-                  auto. auto. auto. 
-                  destruct H3 as [lsf].  destruct H3 as [s'].
-                  remember (current_label sigma) as lb. 
-                  remember (SIGMA s' h) as sigma''.
-                  exists (v_opa_l (ObjId o) lb). exists sigma''. 
-                  apply ST_opaquecall_return2 with (sigma:=sigma) (sigma':=sigma'') (s:=s) (h:=h) (lb:=lb) (s':=s') (lsf:=lsf) (v:=(ObjId o)). 
-                  auto. auto. auto. auto. apply v_oid. 
-
-                  rewrite -> H3 in H2. inversion H2. inversion H5. 
-
-                  subst. 
-                  inversion H. inversion H4.
-
-                  subst. 
-                  remember (SIGMA s h)  as sigma. 
-                  remember (current_label sigma) as lb. 
-                  remember (SIGMA s' h) as sigma'.
-                  exists (v_opa_l (v_l t l0) lb). exists sigma'. 
-                  apply ST_opaquecall_return2 with (sigma:=sigma) (sigma':=sigma') (s:=s) (h:=h) (lb:=lb) (s':=s') (lsf:=lsf) (v:=(v_l t l0)). 
-                  auto. rewrite -> H5 in Heqsigma. inversion Heqsigma. auto. auto. auto. auto. 
-
-
-                  subst. inversion H. inversion H4.
-
-                  subst. 
-                  remember (SIGMA s h)  as sigma. 
-                  remember (current_label sigma) as lb. 
-                  remember (SIGMA s' h) as sigma'.
-                  exists (v_opa_l (v_opa_l t l0) lb). exists sigma'. 
-                  apply ST_opaquecall_return2 with (sigma:=sigma) (sigma':=sigma') (s:=s) (h:=h) (lb:=lb) (s':=s') (lsf:=lsf) (v:=(v_opa_l t l0)). 
-                  auto. rewrite -> H5 in Heqsigma. inversion Heqsigma. auto. auto. auto. auto. 
-                  
-                  (* return label *)
-
-                  exists (opaqueCall(t')). exists sigma'. apply ST_opaquecall1 with (sigma:=(SIGMA s h)) (sigma':=sigma') (e:=e) (e':=t'). 
-                  intros. intro contra. rewrite -> contra in H3. apply H3 with (t:=v). auto. auto.
+                  exists Error_state. apply ST_opaquecall_ctx_error with (sigma:=(SIGMA s h)) (e:=e). auto. 
 
 (* Skip *)
   - left. apply v_none. 
@@ -1300,14 +1312,17 @@ Proof with auto.
 - right. destruct IHhas_type. auto. auto. auto.
                   remember (update_stack_top s x e) as s'.
                   remember (SIGMA s' h) as sigma'.
-                  exists Skip. exists sigma'.
+                  exists (Config Skip sigma').
                   apply ST_assignment2 with (sigma:=sigma) (sigma':=sigma') (id:=x) (v:=e) (s':=s') (s:=s) (h:=h).
                   auto. auto. auto. auto.
 
-                  destruct H4 as [t']. destruct H4 as [sigma'].
-                  exists (Assignment x t'). exists sigma'. 
-                  apply ST_assignment1 with (sigma:=sigma) (sigma':=sigma') (e:=e) (e':=t') (id:=x).
-                  auto. 
+                  destruct H4 as [config']. destruct config'. 
+                  exists (Config (Assignment x t) s0). 
+                  apply ST_assignment1 with (sigma:=sigma) (sigma':=s0) (e:=e) (e':=t) (id:=x).
+                  auto.
+
+                  exists Error_state. 
+                  apply ST_assignment_ctx_error with (sigma:=sigma) (e:=e) (id:=x). auto.  
 
 (* FieldWrite *)
 -right. 
@@ -1325,133 +1340,173 @@ Proof with auto.
             remember (fields_update F f e) as F'. 
             remember (add_heap_obj h o (Heap_OBJ cls_def F' l')) as h'.
             remember (SIGMA s h') as sigma'.
-            exists Skip. exists sigma'.
+            exists (Config Skip sigma').
             apply ST_fieldWrite3 with (sigma:=sigma) (sigma':=sigma') (o:=o) (s:=s) (h:=h) (h':=h') (f:=f) 
                                                       (lb:=lb) (cls:=cls_def) (F:=F) (F':=F') (v:=e) (l':=l').
             auto. auto. auto. auto. auto. auto.  auto.
             
           (* case analysis for argument, if the argument is not a value *)
             subst. 
-                destruct H6 as [t']. destruct H as [sigma'].
+                destruct H6 as [config'].
                 pose proof (excluded_middle_opaqueLabel e).
                 destruct H5.
                   (* case for e = unlabelOpaque t *)
                   destruct H5 as [t]. 
                   rewrite -> H5 in H. inversion H. subst. 
-                  exists (FieldWrite (ObjId o) f (unlabelOpaque e')).
-                  exists (sigma').
+                  exists (Config (FieldWrite (ObjId o) f (unlabelOpaque e')) sigma').
                   apply ST_fieldWrite2 with (sigma:=(SIGMA s h)) (sigma':=sigma') 
                                             (v:=(ObjId o)) (e2:=unlabelOpaque t) (e2':=unlabelOpaque e') (f:=f).
-                  intros. subst. intro contra. inversion contra. rewrite -> H9 in H. inversion H5.
-                      rewrite <- H8 in H; subst; inversion H7. auto.  subst. inversion H7.  subst.
-                      inversion H7. subst. inversion H7. subst. inversion H7. subst. inversion H7.
-                      assumption. assumption. 
-                      subst. 
-                      assert (exists fieldsMap lb, h(o) = Some (Heap_OBJ cls_def fieldsMap lb)).
-                      remember (SIGMA s h ) as sigma.
-                      apply wfe_oid with (o:=o) (ct:=CT) (gamma:=Gamma) (s:=s) (h:=h) 
-                                    (sigma:=sigma) (cls_def:=cls_def) (cn:=clsT). auto. auto. auto. auto.
-                      destruct H5 as [F]. destruct H5 as [lo]. 
-
-                      remember (SIGMA s h ) as sigma.
-                      remember (join_label lo lb) as l'. 
-                      remember (fields_update F f t') as F'. 
-                      remember (add_heap_obj h o (Heap_OBJ cls_def F' l')) as h'.
-                      remember (SIGMA s h') as sigma'.
-                      exists Skip. exists sigma'.
-                      apply ST_fieldWrite_opaque with (sigma:=sigma) (sigma':=sigma') (o:=o) (s:=s) (h:=h) (h':=h') (f:=f) 
-                                                      (lb:=lb) (lo:=lo) (cls:=cls_def) (F:=F) (F':=F') (v:=t') (l':=l').
-                      auto. auto. auto. auto. auto. auto.  auto.
-
-                  (*exception case *)
-                  subst. exists NPE. exists (SIGMA s h).
-                  apply ST_FieldWriteOpaqueDataException with (sigma:=(SIGMA s h)) (o:=o) (f:=f).
-
-                  (* case for argu <> unlabelOpaque t *)
-                  exists (FieldWrite (ObjId o) f t'). exists sigma'. 
-                  apply ST_fieldWrite2 with (sigma:=(SIGMA s h)) (sigma':=sigma') (v:=((ObjId o))) 
-                                            (e2:=e) (e2':=t') (f:=f).
-                  intros. apply H5. apply v_oid. assumption.
-                  rewrite <- H5 in H2_. inversion H2_.
-                  exists NPE. exists sigma.
-                  apply ST_fieldWriteException with (sigma:=sigma) (f:=f) (v:=e).
+                  intros. subst. intro contra. inversion contra. rewrite H8 in H9. 
+                  inversion H5. 
+                  rewrite <- H7 in H9.  inversion H9.                   rewrite <- H7 in H9.  inversion H9. 
+                  rewrite <- H7 in H9.  inversion H9.                   rewrite <- H7 in H9.  inversion H9. 
+                  rewrite <- H7 in H9.  inversion H9.                   rewrite <- H7 in H9.  inversion H9. 
                   auto. auto. 
 
-                  rewrite <- H5 in H2_. inversion H2_.
-                  rewrite <- H5 in H2_. inversion H2_.
-                  rewrite <- H5 in H2_. inversion H2_.
-     
-      + destruct  IHhas_type2.  auto. auto. auto. auto. 
-          destruct H4 as [t']. destruct H4 as [sigma']. 
-          exists (FieldWrite t' f e). exists (sigma').   
-          apply ST_fieldWrite1 with (sigma:=sigma) (sigma':=sigma') (f:=f) (e1:=x) (e1':=t') (e2:=e).
-          auto. 
+                  exists Error_state. subst. apply ST_fieldWrite_ctx_error2 
+                        with (sigma:=(SIGMA s h)) (f:=f) (v:=(ObjId o)) (e2:=(unlabelOpaque t)).
 
-          destruct H4 as [t']. destruct H4 as [sigma']. 
-          exists (FieldWrite t' f e). exists (sigma').   
-          apply ST_fieldWrite1 with (sigma:=sigma) (sigma':=sigma') (f:=f) (e1:=x) (e1':=t') (e2:=e).
-          auto. 
+                  intros. intro contra. inversion contra. rewrite H8 in H9. inversion H5. 
+                  rewrite <- H7 in H9.  inversion H9.                   rewrite <- H7 in H9.  inversion H9. 
+                  rewrite <- H7 in H9.  inversion H9.                   rewrite <- H7 in H9.  inversion H9. 
+                  rewrite <- H7 in H9.  inversion H9.                   rewrite <- H7 in H9.  inversion H9. 
+                  auto. auto. 
+
+                  assert (exists fieldsMap lb, h(o) = Some (Heap_OBJ cls_def fieldsMap lb)).
+                      apply wfe_oid with (o:=o) (ct:=CT) (gamma:=Gamma) (s:=s) (h:=h) 
+                                    (sigma:=sigma) (cls_def:=cls_def) (cn:=clsT). auto. auto. auto. auto.
+                      destruct H13 as [F]. destruct H13 as [lo]. 
+                      remember (fields_update F f v) as F'. 
+                      remember (join_label lo lb) as l''. 
+                      remember (add_heap_obj h o (Heap_OBJ cls_def F' l'')) as h'.
+                      remember (SIGMA s h') as sigma''.
+
+                      exists (Config Skip sigma'').
+                      apply ST_fieldWrite_opaque with (sigma:=(SIGMA s h)) (sigma':=sigma'') (o:=o) (s:=s) (h:=h) (h':=h') (f:=f) 
+                                                      (lb:=lb) (lo:=lo) (cls:=cls_def) (F:=F) (F':=F') (v:=v) (l':=l'') (e2:=e).
+                      rewrite <- H6 in H5. auto. auto. auto. auto. auto. auto.  auto.
+
+                      exists Error_state. 
+
+                      apply ST_fieldWrite_ctx_error2 with (sigma:=(SIGMA s h)) (f:=f) (v:=(ObjId o)) (e2:=e).
+                       intros. rewrite H5. intro contra. inversion contra. rewrite <- H12 in H10.
+                      rewrite H7 in H10. auto. auto. subst. auto.   
+
+                  (* case for argu <> unlabelOpaque t *)
+                  destruct config'. 
+                  exists (Config (FieldWrite (ObjId o) f t) s0). 
+                  apply ST_fieldWrite2 with (sigma:=(SIGMA s h)) (sigma':=s0) (v:=((ObjId o))) 
+                                            (e2:=e) (e2':=t) (f:=f).
+                  intros. apply H5. apply v_oid. assumption.
+
+                  exists Error_state. 
+                      apply ST_fieldWrite_ctx_error2 with (sigma:=(SIGMA s h)) (f:=f) (v:=(ObjId o)) (e2:=e).
+                       intros. apply H5.  auto. auto. 
+     
+                  destruct  IHhas_type2.  auto. auto. auto. 
+                  rewrite <- H5 in H2_. inversion H2_.                   rewrite <- H5 in H2_. inversion H2_.
+  
+                  exists Error_state.
+                  apply ST_fieldWriteException with (sigma:=sigma) (f:=f) (v:=e). 
+
+                  rewrite <- H5 in H2_. inversion H2_.                   rewrite <- H5 in H2_. inversion H2_.
+                  rewrite <- H5 in H2_. inversion H2_.       
+
+
+          +    destruct H4 as [config'].
+                 destruct config'. 
+                  exists (Config (FieldWrite t f e) (s0)). 
+                  apply ST_fieldWrite1 with (sigma:=sigma) (sigma':=s0) (f:=f) (e1:=x) (e1':=t) (e2:=e).
+                  auto. 
+        
+              exists Error_state. 
+              apply ST_fieldWrite_ctx_error1 with (sigma:=sigma) (f:=f) (e1:=x) (e2:=e). auto. 
 
 (* if *)
 - (*destruct  IHhas_type1; auto.  destruct  IHhas_type2; auto. *)
   inversion H2. inversion H1. subst. inversion H3. 
-  assert (exists v1, sf id1 = Some v1). 
+  assert (exists v1, sf id1 = Some v1).
+ 
   apply Typed_variable with (sigma:=(SIGMA (s) h)) (s:=s) (h:=h) (ct:=CT) 
-                                            (gamma:=Gamma) (x:=id1) (T:=(classTy T)) (lb:=lb) (sf:=sf) (s':=s').
+                                            (gamma:=Gamma) (x:=id1) (T:=T) (lb:=lb) (sf:=sf) (s':=s').
   auto. auto. auto. auto. 
   assert (exists v2, sf id2 = Some v2). 
   apply Typed_variable with (sigma:=(SIGMA (s) h)) (s:=s) (h:=h) (ct:=CT) 
-                                            (gamma:=Gamma) (x:=id2) (T:=(classTy T)) (lb:=lb) (sf:=sf) (s':=s').
+                                            (gamma:=Gamma) (x:=id2) (T:=T) (lb:=lb) (sf:=sf) (s':=s').
   auto. auto. auto. auto. 
 
-  destruct H19 as [v1].   destruct H20 as [v2].
-  right. inversion H8. inversion H21. destruct H22 with id1 v1. 
-  rewrite <- H27; auto. destruct H22 with id2 v2.  destruct H22 with id1 v1.  
-  rewrite <- H27; auto. rewrite <- H27; auto. rewrite <- H27; auto. 
-  
-  exists s1. exists sigma.
-  apply ST_if_b1 with (sigma:=sigma) (s1:=s1) (s2:=s2) (v1:=v1) (v2:=v2)
+  destruct H15 as [v1].   destruct H16 as [v2].
+  right. inversion H10.  inversion H17. destruct H18 with T id1. auto. 
+  destruct H18 with T id2. auto.
+    destruct H23. destruct H26. 
+          destruct H27. destruct H28.  
+          exists (Config s1 sigma).
+          apply ST_if_b1 with (sigma:=sigma) (s1:=s1) (s2:=s2) 
                                 (s:=s) (h:=h) (lsf:=lsf) (s':=s') (lb:=lb) (sf:=sf) (id1:=id1) (id2:=id2). 
-  auto. rewrite <- H24 in H4. assumption. auto. auto. auto. subst. auto. 
-  destruct H28.
+  auto. rewrite <- H22 in H4. assumption. auto. auto. auto. subst. auto.
+  rewrite <- H23 in H26. auto. 
 
-  exists s2. exists sigma.
-  apply ST_if_b2 with (sigma:=sigma) (s1:=s1) (s2:=s2) (v1:=v1) (v2:=v2)
+          destruct H28 as [o]. destruct H28. 
+  exists (Config s2 sigma).
+  apply ST_if_b2 with (sigma:=sigma) (s1:=s1) (s2:=s2)
                                 (s:=s) (h:=h) (lsf:=lsf) (s':=s') (lb:=lb) (sf:=sf) (id1:=id1) (id2:=id2). 
-  auto. rewrite <- H24 in H4. assumption. auto. auto. auto. intuition.
-  rewrite -> H25 in H30.  rewrite -> H28 in H30. inversion H30.
-  rewrite -> H25 in H30.  rewrite -> H28 in H30. inversion H30.
-  rewrite -> H25 in H30.  rewrite -> H28 in H30. inversion H30.
-  rewrite -> H25 in H30.  rewrite -> H28 in H30. inversion H30.
+    auto. rewrite <- H22 in H4. assumption. auto. auto. auto. 
+    rewrite <- H25 in H23.     rewrite <- H25 in H26. 
+    rewrite H15 in H23.       rewrite H16 in H26. subst. intro contra. 
+    rewrite contra in H15. rewrite H15 in H16. inversion H16. 
+    rewrite H4 in H23. rewrite H26 in H23. inversion H23. 
 
-
-
-destruct H22 with id2 v2.
-  rewrite <- H27.  auto.
-  exists s2. exists sigma.
-  apply ST_if_b2 with (sigma:=sigma) (s1:=s1) (s2:=s2) (v1:=v1) (v2:=v2)
+    destruct H28. 
+    exists (Config s2 sigma).
+    apply ST_if_b2 with (sigma:=sigma) (s1:=s1) (s2:=s2) 
                                 (s:=s) (h:=h) (lsf:=lsf) (s':=s') (lb:=lb) (sf:=sf) (id1:=id1) (id2:=id2). 
-  auto. rewrite <- H24 in H4. assumption. auto. auto. auto. intuition. 
-  rewrite -> H28 in H29. rewrite -> H30 in H29. inversion H29.
-  rewrite -> H28 in H29. rewrite -> H30 in H29. inversion H29.
-  rewrite -> H28 in H29. rewrite -> H30 in H29. inversion H29.
-  rewrite -> H28 in H29. rewrite -> H30 in H29. inversion H29.
+    auto. rewrite <- H22 in H4. assumption. auto. 
+    destruct H27 as [o]. destruct H27. 
+    intro contra. 
+    rewrite  H25 in contra. rewrite contra in H23. rewrite H26 in H23. 
+    rewrite H27 in H23. rewrite H28 in H23. inversion H23. 
 
-destruct H28. destruct H25.  
+    (*case analysis*)
+    
 
-exists s1. exists sigma.
-  apply ST_if_b1 with (sigma:=sigma) (s1:=s1) (s2:=s2) (v1:=v1) (v2:=v2)
-                                (s:=s) (h:=h) (lsf:=lsf) (s':=s') (lb:=lb) (sf:=sf) (id1:=id1) (id2:=id2). 
-  auto. rewrite <- H24 in H4. assumption. auto. auto. auto. rewrite -> H28. auto.
+          destruct H28 as [o]. destruct H27 as [o'].
+          case_eq (beq_oid o o'). intro. 
+          assert (o=o').
+          apply beq_oid_equal with (x:=o) (x':=o'). auto. 
+          destruct H27. destruct H28. rewrite H30 in H28. rewrite <- H28 in H27.
+          rewrite H27 in H23. rewrite <- H26 in H23. rewrite <- H25 in H23. 
+
+          exists (Config s1 sigma ).
+          apply ST_if_b1 with (sigma:=sigma) (s1:=s1) (s2:=s2)
+                                (s:=s ) (h:=h) (lsf:=lsf) (s':=s') (lb:=lb) (sf:=sf) (id1:=id1) (id2:=id2). 
+          auto.  rewrite <- H22 in H4. assumption. auto. auto. auto.
+
+          intro. destruct H27. destruct H28.
+          assert (Some x1 <> Some x0).  intro contra. inversion contra.  
+          rewrite <- H33 in H27. rewrite H27 in H28.
+          inversion H28. assert (beq_oid o o' = true). rewrite H34. apply beq_oid_same. 
+          rewrite H32 in H29. inversion H29.
+
+          rewrite <- H26 in H32. rewrite <- H23 in H32. rewrite <- H25 in H32.
+          exists (Config s2 sigma ).
+          apply ST_if_b2 with (sigma:=sigma) (s1:=s1) (s2:=s2)
+                                (s:=s ) (h:=h) (lsf:=lsf) (s':=s') (lb:=lb) (sf:=sf) (id1:=id1) (id2:=id2). 
+          auto.  rewrite <- H22 in H4. assumption. auto. auto. 
+          
 
 (* sequence *)
 - right. destruct IHhas_type1. auto. auto. auto.
-   exists e2. exists sigma. 
+    exists (Config e2 sigma).
+   
    apply ST_seq2 with (sigma:=sigma) (v:=e1) (s:=e2); auto.
   
-  destruct H2 as [t']. destruct H2 as [sigma'].
-  exists (Sequence t' e2). exists sigma. 
-   apply ST_seq1 with (sigma:=sigma) (s1:=e1) (s2:=e2) (s1':=t'); auto.
+  destruct H2 as [config'].
+  destruct config'.
+  exists (Config (Sequence t e2) s0). 
+   apply ST_seq1 with (sigma:=sigma) (s1:=e1) (s2:=e2) (s1':=t); auto.
+
+  exists Error_state. apply ST_seq_ctx_error with (sigma:=sigma) (s1:=e1) (s2:=e2).
+  auto. 
 
 (* return e *)
 - right. destruct IHhas_type. auto. auto. auto. 
@@ -1462,14 +1517,17 @@ exists s1. exists sigma.
   remember (join_label (get_current_label s) (get_current_label s')) as l'.
   remember (update_current_label s' l' ) as s''.
   remember (SIGMA s'' h) as sigma'.
-  exists e. exists sigma'.
+  exists (Config e sigma').
   apply ST_return2 with (sigma:=sigma) (sigma':=sigma') (v:=e)
                                     (s:=s) (s':=s') (s'':=s'') (h:=h) (lsf:=lsf) (l':=l').
   auto. auto. auto. auto. auto. auto. 
 
-  destruct H4 as [t']. destruct H4 as [sigma'].
-  exists (Return t'). exists sigma'. 
-  apply ST_return1 with (sigma:=sigma) (sigma':=sigma') (e:=e) (e':=t'). auto.
+  destruct H4 as [config'].
+  destruct config'. 
+  exists (Config (Return t) s0). 
+  apply ST_return1 with (sigma:=sigma) (sigma':=s0) (e:=e) (e':=t). auto.
+
+  exists Error_state. apply ST_return_ctx_error with (sigma:=sigma) (e:=e). auto. 
 
 (* ObjId o *)
 - left. apply v_oid. 
@@ -1481,75 +1539,674 @@ exists s1. exists sigma.
 - left. apply v_opa_labeled.
 Qed.
 
+
+Check progress. 
+
 (* reduction preserve well-form of stack and heap *)
-Theorem reduction_preserve_wfe : forall t t' T  sigma sigma' gamma CT s s' h h', 
-    sigma = SIGMA s h ->  wfe_heap CT gamma h -> wfe_stack CT gamma h s -> 
-    has_type CT gamma h t T -> 
-    t / sigma ==> t' / sigma' ->
-    sigma' = SIGMA s' h' ->
+Theorem reduction_preserve_wfe : forall gamma CT s s' h h' sigma sigma',
+    sigma = SIGMA s h ->  wfe_heap CT gamma h -> wfe_stack CT gamma h s ->
+     sigma' = SIGMA s' h' -> 
+    forall t T, has_type CT gamma h t T -> 
+     forall t',  Config t sigma ==> Config t' sigma' ->
     wfe_heap CT gamma h' /\ wfe_stack CT gamma h' s'.
-Proof with auto. 
+Proof. 
+    intros gamma CT s s' h h' sigma sigma'. 
+    intro. intro. intro. intro. 
+    induction t. (*induction on the terms *)
+  (* (Tvar i) *)
+  + intro T. intro typing. intro t'.  intro step. inversion step.
+      rewrite H in H6. rewrite H2 in H6. inversion H6. 
+      rewrite <- H12. rewrite <- H13.
+      split. auto. auto.
+  (* null *)
+  + intro T. intro typing. intro t'.  intro step. inversion step.
+  (* field access *)
+  + intro T. intro typing. intro t'.  intro step. 
+      inversion step.  inversion typing.
+      apply IHt with (T:=(classTy clsT)) (t':=e'). auto. auto.
+      (*subgoal#2 *)      
+      inversion typing. subst. inversion H13. inversion H8. 
+      split.       rewrite <- H5. auto.
+      rewrite <- H5. rewrite <- H4. 
+      remember (join_label lb (current_label (SIGMA s h))) as lb'.
+      unfold update_current_label.
+      inversion H1.
+ 
+      
 Admitted. 
 
 
-(* reduction preserve typing *)
 
-Theorem preservation : forall t t' T  sigma sigma' gamma CT s s' h h', 
+(* types of variable in stack are consistent with the object identifiers that they are pointing to.  *)
+Lemma stack_frame_preserve_typing : forall sigma gamma CT s h x o s' cls_name  cls_name' method_defs field_defs lb sf cls_def F, 
     sigma = SIGMA s h ->  wfe_heap CT gamma h -> wfe_stack CT gamma h s -> 
-    has_type CT gamma h t T -> 
-    t / sigma ==> t' / sigma' ->
-    sigma' = SIGMA s' h' ->
-    exists T', has_type CT gamma h' t' T'.
+    (s = cons (Labeled_frame lb sf) s') ->
+    (sf x = Some (ObjId o)) -> 
+    h(o) = Some (Heap_OBJ cls_def F lb) -> 
+    cls_def = class_def cls_name' field_defs method_defs ->
+    gamma x = Some (classTy cls_name) -> cls_name' = cls_name.
+Proof.
+    intros. inversion H1. rewrite H8 in H4.  inversion H4.
+    subst. inversion H12. destruct H2 with cls_name x. auto. destruct H16. 
+      destruct H17. subst. inversion H7. inversion H. subst. rewrite H3 in H16. inversion H16. 
+
+    destruct H17. destruct H17. destruct H18 as [F0]. 
+         destruct H18 as [lx]. destruct H18 as [field_defs0]. destruct H18 as [method_defs0]. 
+    destruct H18. subst. inversion H7. inversion H. subst. rewrite H3 in H16.  inversion H16.
+    rewrite <- H13 in H18. rewrite H4 in H18. inversion H18. auto. 
+Qed.
+
+Lemma field_consist_typing : forall CT gamma v h o cls_def F f lb field_cls_name cls_name field_defs method_defs,
+  wfe_heap CT gamma h -> 
+  h(o) = Some (Heap_OBJ cls_def F lb) -> 
+  cls_def = class_def cls_name field_defs method_defs ->
+  type_of_field field_defs f = Some field_cls_name ->
+  F f = Some v ->
+     ( v = null \/ 
+          ( exists o' field_defs0 method_defs0 field_cls_def F' lo, 
+           v = (ObjId o') 
+          /\ field_cls_def = (class_def field_cls_name field_defs0 method_defs0) 
+          /\ h(o') = Some (Heap_OBJ field_cls_def F' lo) 
+          /\ CT field_cls_name = Some field_cls_def 
+          )
+      ).
+Proof with auto. 
+  intros. induction H. inversion H0.
+  case_eq (beq_oid o0 o). intro. rewrite H6 in H0. rewrite H11 in H0. 
+  rewrite H0 in H5.  inversion H5. rewrite <- H13 in H8.
+rewrite H1 in H8. inversion H8. 
+  destruct H9 with  f field_cls_name. rewrite <- H17. auto. 
+  rewrite <- H14 in H12.  destruct H12. rewrite H3 in H12.  inversion H12. 
+  destruct H19. 
+
+  left. auto.
+  right. destruct H19 as [o']. destruct H19 as [F']. destruct H19 as [lx].
+     destruct H19 as [field_defs']. destruct H19 as [method_defs'].
+     exists o'. exists  field_defs'. exists method_defs'. 
+     exists (class_def field_cls_name field_defs' method_defs'). 
+     exists F'. exists lx. 
+
+    destruct H19.     destruct H20. 
+    split. auto. split. auto. auto. 
+
+
+    intro.  
+    assert (
+             v = null \/
+             (exists
+                (o' : oid) (field_defs0 : list field) (method_defs0 : 
+                                                       list method_def) 
+              (field_cls_def : CLASS) (F' : FieldMap) (lo : Label),
+                v = ObjId o' /\
+                field_cls_def =
+                class_def field_cls_name field_defs0 method_defs0 /\
+                h o' = Some (Heap_OBJ field_cls_def F' lo) /\
+                ct field_cls_name = Some field_cls_def)).
+ apply  IHwfe_heap. auto.
+rewrite H6 in  H0. rewrite H11 in H0. auto. auto. 
+
+
+ destruct H12. left. auto. 
+
+  right.
+
+ destruct H12 as [o']. destruct H12 as [field_defs']. 
+destruct H12 as [method_defs'].
+destruct H12 as [field_cls_def'].
+destruct H12 as [F']. destruct H12 as [lx].
+destruct H12. destruct H13. destruct H14. 
+
+ case_eq  (beq_oid o0 o'). intro. 
+exists o0. exists field_defs. exists method_defs. 
+exists field_cls_def'. exists F. exists lb. 
+
+
+assert (o0=o').
+ apply beq_oid_equal with (x:=o0) (x':=o'). auto. rewrite H17. 
+rewrite <- H17 in H14. rewrite  H in H14. inversion H14.
+
+
+intro.  
+     exists o'. exists  field_defs'. exists method_defs'.
+     exists (class_def field_cls_name field_defs' method_defs'). 
+     exists F'. exists lx.
+split. auto. split. auto. split.  rewrite H6. rewrite H16.  rewrite H13 in H14. auto. rewrite H13 in H15. auto.  
+Qed. 
+
+
+
+
+Lemma heap_preserve_typing : forall h h' t T CT gamma,
+(forall o cls_def F lo, h o = Some  (Heap_OBJ cls_def F lo) 
+                              -> exists F' lo', h' o = Some  (Heap_OBJ cls_def F' lo') )
+ -> has_type CT gamma h t T -> has_type CT gamma h' t T.
+Proof. 
+  intros h h' t T CT gamma. 
+  intro Hyh.
+  intro Hy.  
+  induction Hy. 
+  + apply T_Var. auto. 
+  + apply T_null.
+  + apply T_FieldAccess with (cls_def:=cls_def) (clsT:=clsT) 
+            (fields_def:=fields_def); auto. 
+  + apply T_MethodCall with (T:=T) (cls_def:=cls_def) (body:=body) (arg_id:=arg_id)
+        (arguT:=arguT) (para_T:=para_T) (cls_a:=cls_a); auto.
+  + apply T_NewExp with (cls_def:=cls_def). auto. apply H0.
+  + apply T_label.
+  + apply T_labelData; auto.
+  + apply T_unlabel; auto.
+  + apply T_labelOf with (T:=T); auto. 
+  + apply T_unlabelOpaque. auto.
+  + apply T_opaqueCall. auto.
+  + apply T_skip.
+  + apply T_assignment with (T:=T); auto. 
+  + apply T_FieldWrite with (cls_def:=cls_def) (clsT:=clsT) (cls':=cls'); auto. 
+  + apply T_if with (T:=T); auto.
+  + apply T_sequence with (T:=T); auto.
+  + apply T_return; auto. 
+  + apply T_ObjId with (cls_def:=cls_def). 
+    auto. destruct H0 as [F]. destruct H0 as [lo].
+    
+    destruct Hyh with (o:=o) (cls_def:=cls_def) (F:=F) (lo:=lo).
+    auto. destruct H2 as [lx]. exists x. exists lx. auto. auto. 
+  + apply T_v_l; auto.
+  + apply T_v_opa_l; auto.
+Qed. 
+
+
+
+Lemma reduction_preserve_heap_pointer : forall t s s' h h', 
+     forall CT gamma T, has_type CT gamma h t T ->
+     forall t', reduction (Config t (SIGMA s h)) (Config t' (SIGMA s' h')) -> 
+     (forall o cls_def F lo, h o = Some  (Heap_OBJ cls_def F lo) 
+                              -> exists F' lo', h' o = Some  (Heap_OBJ cls_def F' lo') ).
+Proof.
+     intros  t s s' h h'.
+     intros CT gamma. 
+     induction t; intro T; intro typing; intro t'; intro step; inversion step; inversion typing. 
+     + intuition. exists F. exists lo. auto.  
+     + apply IHt with  (classTy clsT) e'; auto.
+     + inversion H9. auto. 
+          inversion H4. auto.  intuition. exists F. exists lo. auto. 
+     + apply IHt1 with (classTy T0) e'; auto.
+     + apply IHt2 with arguT e'; auto.
+     + inversion H14. auto.  intuition. exists F. exists lo. auto.  
+     + inversion H12. auto.   intuition. exists F. exists lo. auto.  
+     + unfold add_heap_obj in H7. inversion H9. rewrite H8. 
+        intuition.
+        case_eq (beq_oid o o0). intro.  auto.  inversion H3. rewrite H23 in H17. 
+        apply beq_oid_equal with (x:=o) (x':=o0) in H20. 
+        rewrite H20 in H4. rewrite H4 in H17. inversion H17.
+ 
+        intro. inversion H3.  auto.  intuition. exists F0. exists lo. auto. 
+        rewrite H23 in H17. unfold add_heap_obj. rewrite H20. auto.
+
+     + apply IHt with T0 e'; auto. 
+     + auto.  intuition. exists F. exists lo. auto.  
+     + apply IHt with (LabelelTy T) e'; auto. 
+     + inversion H6. auto.  intuition. exists F. exists lo. auto.   
+     + apply IHt with (LabelelTy T0) e'; auto. 
+     + auto.  intuition. exists F. exists lo. auto.  
+     + apply IHt with (OpaqueLabeledTy T) e'; auto. 
+     + inversion H6. auto.  intuition. exists F. exists lo. auto.   
+     + apply IHt with T0 e'; auto. 
+     + subst.  apply IHt with T0 (Return e'). auto. apply ST_return1. auto.
+     + auto.  intuition. exists F. exists lo. auto.  
+     + subst. inversion H3. inversion H6. auto.  intuition. exists F. exists lo. auto.   
+     + apply IHt with T0 e'; auto. 
+     + inversion H5. inversion H7. auto.  intuition. exists F. exists lo. auto.   
+     + apply IHt1 with (classTy clsT) e1'; auto.
+     + apply IHt2 with  (classTy cls') e2'; auto.
+     + inversion H10. rewrite H9.  unfold add_heap_obj. inversion H5. 
+        intros o0 cls_def0 F0 lx. 
+        case_eq (beq_oid o o0). intro. 
+        apply beq_oid_equal with (x:=o) (x':=o0) in H23. 
+        intro. rewrite <- H23 in H28. rewrite <- H6 in H28. inversion H28. 
+        exists F'. exists l'. auto. 
+
+        intro. intro. exists F0. exists lx. auto.  
+     + inversion H11. rewrite H10.  unfold add_heap_obj. inversion H6. 
+        intros o0 cls_def0 F0 lx. 
+        case_eq (beq_oid o o0). intro. 
+        apply beq_oid_equal with (x:=o) (x':=o0) in H23. 
+        intro. rewrite <- H23 in H28. rewrite <- H7 in H28. inversion H28. 
+        exists F'. exists l'. auto. 
+
+        intro. intro. exists F0. exists lx. auto.  
+
+     + intuition. exists F. exists lo. auto. 
+     + intuition. exists F. exists lo. auto.
+     + apply IHt1 with T0 s1'; auto.
+     + intuition. exists F. exists lo. auto. 
+     + apply IHt with T e'; auto.
+     + intuition. exists F. exists lo. inversion H8. inversion H4. rewrite <-H21. auto. 
+Qed.
+
+Theorem preservation : forall gamma CT s s' h h' sigma sigma',
+    sigma = SIGMA s h ->  wfe_heap CT gamma h -> wfe_stack CT gamma h s -> sigma' = SIGMA s' h' -> 
+    forall t T, has_type CT gamma h t T -> 
+     forall t',  Config t sigma ==> Config t' sigma' ->
+     ( has_type CT gamma h' t' T) .
 Proof with auto.
-   intros. 
+   intros gamma CT s s' h h' sigma sigma'. 
+  intro. intro. intro. intro. 
+  induction t. (*induction on the terms *)
+  (* (Tvar i) *)
+  + intro T. intro typing. intro t'.  intro step.
+        inversion step.   inversion typing. subst. 
+        assert ( ( t' = null \/ 
+                 ( exists o, t' = ObjId o 
+                              /\ gamma i = Some (classTy T0)
+                              /\ (exists F lo field_defs method_defs , h(o) = Some (Heap_OBJ (class_def T0 field_defs method_defs) F lo)
+                                      /\ (CT T0 = Some (class_def T0 field_defs method_defs))
+                                   ) 
+                  )    ) ).
+      inversion H6. inversion H1.   rewrite H5 in H15. inversion H15.
+      inversion H11. destruct H18 with T0 i. auto. subst. destruct H23. 
+      inversion H7. inversion H17. rewrite <- H20 in H.  rewrite H13 in H.
+      rewrite H in H10. inversion H10. rewrite <- H16. intuition. destruct H3.
+      right. exists x1. destruct H2. split; auto. 
+
+      destruct H. rewrite H. apply T_null with (Gamma:=gamma) (h:=h') (T:=(classTy T0)) (CT:=CT).
+
+      destruct H.  destruct H. destruct H2. destruct H3 as [F]. destruct H3 as [lo]. 
+      destruct H3 as [field_defs]. destruct H3 as [method_defs]. destruct H3. rewrite H.  
+      apply T_ObjId with (h:=h') (Gamma:=gamma) (CT:=CT) (o:=x) (cls_name:=T0)
+                       (cls_def:=(class_def T0 field_defs method_defs)). auto. 
+      auto. exists F. exists lo. auto.  inversion H6. rewrite <- H9. auto. 
+      exists  field_defs. exists method_defs. auto. 
+
+  (* null *)
+  + intro T. intro typing. intro t'.  intro step.
+        inversion step.  
+
+  (* field access *)
+  + intro T'. intro typing. intro t'. inversion typing. intro step. 
+     inversion step. subst. apply T_FieldAccess with (Gamma:=gamma) (e:=e') (f:=i) 
+            (cls_def:=cls_def) (CT:=CT) (clsT:=clsT) (cls':=cls') (h:=h') 
+            (fields_def:=(find_fields cls_def)). apply IHt. 
+             auto. auto. auto. auto. auto.
+
    assert (wfe_heap CT gamma h' /\ wfe_stack CT gamma h' s').
-   apply reduction_preserve_wfe with (t:=t) (t':=t') (T:=T)  (sigma:=sigma) (sigma':=sigma') (gamma:=gamma) (CT:=CT) (s:=s) (s':=s') (h:=h) (h':=h').
-   auto. auto. auto. auto. auto. auto.  
-    intros. induction H3.
-- (* Tvar *)
-   inversion H2. inversion H1. rewrite -> H17 in H13. inversion H13. 
-   inversion H18.   destruct H30 with id0 v. inversion H29. inversion H3. 
-      subst. inversion H33. intuition.
+   apply reduction_preserve_wfe with (t:=(FieldAccess t i)) (t':=t') (T:=T')  (sigma:=sigma) (sigma':=sigma') (gamma:=gamma) (CT:=CT) (s:=s) (s':=s') (h:=h) (h':=h').
+   auto. auto. auto. auto. auto. auto.   
 
-   exists (classTy T1). rewrite -> H33.
-   apply T_null  with (Gamma:=gamma) (h:=h') (T:= (classTy T1)) (CT:=CT).
+   rewrite <- H13 in H5. inversion H5. 
 
-   destruct H33.  subst. 
+   destruct H32 as [field_defs]. destruct H32 as [method_defs].
+      assert (v = null \/
+             (exists
+                (o' : oid) (field_defs0 : list field) (method_defs0 : 
+                                                       list method_def) 
+              (field_cls_def : CLASS) (F' : FieldMap) (lo : Label),
+                v = ObjId o' /\
+                field_cls_def =
+                class_def cls' field_defs0 method_defs0 /\
+                h' o' = Some (Heap_OBJ field_cls_def F' lo) /\
+                CT cls' = Some field_cls_def)
+      ).
 
-    destruct H34 as [F]. destruct H as [lx]. destruct H as [cls_def0].
+    apply field_consist_typing with (CT:=CT) (gamma:=gamma) (v:=v) (h:=h') (o:=o) (cls_def:=cls)
+             (F:=fields) (f:=i) (lb:=lb) (field_cls_name:=cls') (cls_name:=cls_name) 
+             (field_defs:=field_defs) (method_defs:=method_defs).
+    apply H24. rewrite H2 in H23. inversion H23. auto. subst. 
+    inversion H18. rewrite <- H3 in H19. rewrite <- H19 in H31.
+    inversion H31. auto. rewrite <- H6 in H27. inversion H27.
+    destruct H31 as [F]. destruct H as [lx]. inversion H.  auto. 
+    rewrite <- H6 in H27. inversion H27. rewrite <- H34 in H10.
+    rewrite H32 in H10. unfold find_fields in H10.
+    rewrite H10 in H12. auto. subst. auto. 
 
-assert  (exists cn cls_def, CT cn = Some (cls_def)).
-exists T1. exists cls_def. auto.
+    destruct H33. 
+    subst. apply T_null with (Gamma:=gamma) (h:=h') (T:=(classTy cls')) (CT:=CT). 
 
-assert (exists cn field_defs method_defs, CT cn = Some cls_def0 /\ cls_def0 = (class_def cn field_defs method_defs)).
-
-
-apply heap_consist_ct with (h:=h) (o:=o) (ct:=CT) 
-     (ctx:=(fun x' : id => if beq_id x0 x' then Some (classTy T1) else gamma0 x0))
-     (cls:=cls_def0) (F:=F) (lo:=lx).
-auto.  auto.
-
-destruct H7 as [cls_name]. destruct H7 as [field_defs].  destruct H7 as [method_defs].  destruct H7.  
-
-induction cls_def0.
-exists (classTy c). 
-apply T_ObjId with (h:=h') 
-(Gamma:=((fun x' : id => if beq_id x0 x' then Some (classTy T1) else gamma0 x0))) (CT:=CT) (o:=o) 
-                                          (cls_name:=c) (F:=F) (lo:=lx) (cls_def:=(class_def c l0 l1)).
-auto. inversion H9. rewrite <- H9.  auto. 
-inversion H4. rewrite <- H12. auto. 
-
-- (* FieldAccess *)
-inversion H2. 
+    destruct H33 as [o']. destruct H33 as [field_defs0]. destruct H33 as [method_defs0]. 
+    destruct H33 as [field_cls_def]. destruct H33 as [F']. destruct H33 as [lx]. 
+    destruct H33. subst. destruct H34. destruct H2. 
 
 
-  | T_FieldAccess : forall Gamma e f cls_def CT clsT cls' h fields_def,
-      has_type CT Gamma h e (classTy clsT) ->       
-      Some cls_def = CT(clsT) ->
-      fields_def = (find_fields cls_def) ->
-      type_of_field fields_def f = Some cls' ->
-      has_type CT Gamma h (FieldAccess e f) (classTy cls')
+    apply T_ObjId with (h:=h') (Gamma:=gamma) (CT:=CT) (cls_name:=cls') 
+                                  (cls_def:=field_cls_def) (o:=o').
+
+     auto. auto.  exists  F'. exists lx. auto. 
+
+     exists field_defs0. exists method_defs0. auto. 
+
+  (* MethodCall  *)
+    + intro T'. intro typing. intro t'. inversion typing. intro step. 
+        inversion step. 
+      (* reduction on the object  *)
+        - apply T_MethodCall with (Gamma:=gamma) (e:=e') (meth:=i) (argu:=t2)
+                            ( CT:=CT) (h:=h') (T:=T) (returnT:=returnT) (cls_def:=cls_def)
+                            (body:=body) (arg_id:=arg_id) (arguT:=arguT) (para_T:=para_T)
+                          (cls_a:=cls_a) .
+
+      apply IHt1; auto. 
+
+      apply heap_preserve_typing with (h:=h).
+      intros o cls_def0 F lo. intro.  
+
+      apply reduction_preserve_heap_pointer with (t:=t1) (s:=s) (s':=s') (h:=h) (h':=h')
+                             (CT:=CT) (gamma:=gamma) (T:=(classTy T))
+                              (t':=e') (F:=F) (lo:=lo); auto. 
+      rewrite <- H. rewrite <- H2.  auto.  auto. auto. auto. auto. auto. 
+      apply heap_preserve_typing with (h:=h).
+      intros o cls_def0 F lo. intro.  
+      apply reduction_preserve_heap_pointer with (t:=t1) (s:=s) (s':=s') (h:=h) (h':=h')
+                             (CT:=CT) (gamma:=gamma) (T:=(classTy T))
+                              (t':=e') (F:=F) (lo:=lo); auto. 
+      rewrite <- H. rewrite <- H2.  auto.  auto. 
+      (* reduction on the argument  *)
+        -  apply T_MethodCall with (Gamma:=gamma) (e:=t1) (meth:=i) (argu:=e')
+                    ( CT:=CT) (h:=h') (T:=T) (returnT:=returnT) (cls_def:=cls_def)
+                            (body:=body) (arg_id:=arg_id) (arguT:=arguT) (para_T:=para_T)
+                          (cls_a:=cls_a).
+          apply heap_preserve_typing with (h:=h).
+          intros o cls_def0 F lo. intro. 
+
+          apply reduction_preserve_heap_pointer with (t:=t2) (s:=s) (s':=s') (h:=h) (h':=h')
+                                 (CT:=CT) (gamma:=gamma) (T:=arguT)
+                                  (t':=e') (F:=F) (lo:=lo); auto. 
+          rewrite <- H. rewrite <- H2.  auto.  auto. auto. auto. auto. auto. 
+
+          apply heap_preserve_typing with (h:=h).
+          intros o cls_def0 F lo. intro. 
+
+          apply reduction_preserve_heap_pointer with (t:=t2) (s:=s) (s':=s') (h:=h) (h':=h')
+                                 (CT:=CT) (gamma:=gamma) (T:=arguT)
+                                  (t':=e') (F:=F) (lo:=lo); auto. 
+          rewrite <- H. rewrite <- H2.  auto.  auto. 
+      (* normal return  *)
+          -  apply heap_preserve_typing with (h:=h).
+          intros o0 cls_def0 F0 lo0. intro. 
+
+          apply reduction_preserve_heap_pointer with (t:=(MethodCall t1 i t2)) (s:=s) (s':=s') (h:=h) (h':=h')
+                                 (CT:=CT) (gamma:=gamma) (T:=T')
+                                  (t':=t') (F:=F0) (lo:=lo0); auto. 
+          rewrite <- H. rewrite <- H2.  auto. subst.  auto.
+
+          inversion H6. inversion H22. destruct H10 as [F']. destruct H10 as [lo'].
+         rewrite H16 in H10. rewrite H10 in H23. inversion H23. rewrite <- H17 in H3. 
+          rewrite <- H3 in H8. inversion H8. rewrite <- H20 in H24. rewrite H12 in H24. 
+          inversion H24. rewrite <- H16. apply T_return. auto. intuition. inversion H13.   
+      (* opaque return  *)
+      - subst. apply heap_preserve_typing with (h:=h).
+          intros o0 cls_def0 F0 lo0. intro. 
+
+          apply reduction_preserve_heap_pointer with 
+                    (t:=(MethodCall (ObjId o) i (unlabelOpaque (v_opa_l v lb))))
+                     (s:=s) (s':=s') (h:=h) (h':=h')
+                                 (CT:=CT) (gamma:=gamma) (T:= (classTy returnT))
+                                  (t':=(Return body0)) (F:=F0) (lo:=lo0); auto. 
+
+          inversion H6. inversion H22. destruct H10 as [F']. destruct H10 as [lo'].
+         rewrite H16 in H10. rewrite H10 in H23. inversion H23. rewrite <- H17 in H3. 
+         rewrite <- H3 in H8. inversion H8. rewrite H20 in H12.  rewrite H12 in H28. 
+         inversion H28. rewrite <- H16.  apply T_return. auto. intuition. inversion H13.   
+
+(* new expression  *)
+    + intro T. intro typing. intro t'.  intro step. 
+   assert (wfe_heap CT gamma h' /\ wfe_stack CT gamma h' s').
+   apply reduction_preserve_wfe with (t:=(NewExp c)) (t':=t') (T:=T)  (sigma:=sigma)
+           (sigma':=sigma') (gamma:=gamma) (CT:=CT) (s:=s) (s':=s') (h:=h) (h':=h').
+   auto. auto. auto. auto. auto. auto.   
+      inversion step. inversion typing. 
+      apply T_ObjId with (h:=h') (Gamma:=gamma) (CT:=CT) (o:=o)
+                (cls_name:=c) (cls_def:=cls). 
+      assert (h' o = Some (Heap_OBJ cls F lb)).
+      rewrite H2 in H14.       inversion H14.  rewrite H13.       unfold add_heap_obj. 
+      assert (beq_oid o o = true). apply beq_oid_same. rewrite H22. auto.
+      assert (exists cls_name field_defs method_defs, 
+                CT cls_name = Some cls /\ cls = (class_def cls_name field_defs method_defs)).
+      apply heap_consist_ct with (h:=h') (o:=o) (ctx:=gamma) (F:=F) (lo:=lb).
+      apply H3. auto. destruct H23 as [cls_name'].
+      destruct H23 as [field_defs'].       destruct H23 as [method_defs']. destruct H23. 
+      rewrite H10 in H24. inversion H24.  auto. exists F. exists lb.  
+
+      rewrite H2 in H14.       inversion H14.  rewrite H13.       unfold add_heap_obj. 
+      assert (beq_oid o o = true). apply beq_oid_same. rewrite H22. auto.
+      exists field_defs. exists method_defs. auto.
+
+(* Label  *)
+    + intro T. intro typing. intro t'.  intro step. 
+       inversion step. 
+ 
+(* label data *)
+    + intro T. intro typing. intro t'.  intro step.
+        inversion step.   inversion typing.
+        apply T_labelData with (h:=h') (Gamma:=gamma) (lb:=l0) (CT:=CT) (e:=e') (T:=T0).
+        apply T_label. apply IHt; auto. inversion typing.
+        apply T_v_l with (h:=h') (Gamma:=gamma) (lb:=l0) (CT:=CT) (v:=t) (T:=T0).
+        apply T_label. 
+        apply heap_preserve_typing with (h:=h).
+          intros o0 cls_def0 F0 lo0. intro. 
+        apply reduction_preserve_heap_pointer with 
+                    (t:=(labelData t l0))
+                     (s:=s) (s':=s') (h:=h) (h':=h')
+                                 (CT:=CT) (gamma:=gamma) (T:= T)
+                                  (t':=t') (F:=F0) (lo:=lo0); auto.
+        rewrite <- H.         rewrite <- H2. auto. auto.
+
+(* unlabel *)
+    + intro T. intro typing. intro t'.  intro step.
+        inversion step.   inversion typing.
+        apply T_unlabel. apply IHt. auto. auto.
+        inversion typing. rewrite <- H3 in H15. inversion H15. 
+        apply heap_preserve_typing with (h:=h).
+          intros o0 cls_def0 F0 lo0. intro. 
+        apply reduction_preserve_heap_pointer with 
+                    (t:=(unlabel t) )
+                     (s:=s) (s':=s') (h:=h) (h':=h')
+                                 (CT:=CT) (gamma:=gamma) (T:= T)
+                                  (t':=t') (F:=F0) (lo:=lo0); auto.
+        rewrite <- H.         rewrite <- H2. auto. rewrite <- H5. auto. 
+
+(* Label of  *)
+   + intro T. intro typing. intro t'.  intro step.
+        inversion step.   inversion typing.
+        apply T_labelOf with (T:=T0).  apply IHt. auto. auto. 
+        inversion typing. apply T_label.
+
+(* unlabelopaque  *)
+   + intro T. intro typing. intro t'.  intro step.
+        inversion step.   inversion typing.
+        apply T_unlabelOpaque. apply IHt. auto. auto.
+        inversion typing. rewrite <- H3 in H15. inversion H15. rewrite <- H5.  
+        apply heap_preserve_typing with (h:=h).
+          intros o0 cls_def0 F0 lo0. intro. 
+        apply reduction_preserve_heap_pointer with 
+                    (t:=(unlabelOpaque t) )
+                     (s:=s) (s':=s') (h:=h) (h':=h')
+                                 (CT:=CT) (gamma:=gamma) (T:= T)
+                                  (t':=t') (F:=F0) (lo:=lo0); auto.
+        rewrite <- H.         rewrite <- H2. auto. auto. 
+
+(* opaque call  *)
+   + intro T. intro typing. intro t'.  intro step.
+        inversion step.   inversion typing.
+        apply T_opaqueCall. apply IHt. auto. auto.
+        inversion typing. 
+              apply T_opaqueCall. apply IHt. auto. rewrite <- H3.
+        apply ST_return1. auto.
+        inversion typing.  apply T_v_opa_l. apply T_label.
+        apply heap_preserve_typing with (h:=h).
+          intros o0 cls_def0 F0 lo0. intro. 
+        apply reduction_preserve_heap_pointer with 
+                    (t:=(opaqueCall t) )
+                     (s:=s) (s':=s') (h:=h) (h':=h')
+                                 (CT:=CT) (gamma:=gamma) (T:= T)
+                                  (t':=t') (F:=F0) (lo:=lo0); auto.
+        rewrite <- H.         rewrite <- H2. auto. auto. 
+
+        inversion typing.  apply T_v_opa_l. apply T_label.
+        apply heap_preserve_typing with (h:=h).
+          intros o0 cls_def0 F0 lo0. intro. 
+        apply reduction_preserve_heap_pointer with 
+                    (t:=(opaqueCall t) )
+                     (s:=s) (s':=s') (h:=h) (h':=h')
+                                 (CT:=CT) (gamma:=gamma) (T:= T)
+                                  (t':=t') (F:=F0) (lo:=lo0); auto.
+        rewrite <- H.         rewrite <- H2. auto. 
+        rewrite <- H3 in H16. inversion H16. auto. 
+
+(* skip  *)
+   + intro T. intro typing. intro t'.  intro step.
+        inversion step.  
+
+(* assignment  *)
+   + intro T. intro typing. intro t'.  intro step.
+        inversion step.    inversion typing.
+        apply T_assignment with (T:=T0). auto. 
+        apply IHt. auto. auto. 
+        inversion typing. apply T_skip.
+
+(* field write  *)
+   + intro T. intro typing. intro t'.  intro step.
+        inversion step.    inversion typing.
+        apply T_FieldWrite with (cls_def:=cls_def) (clsT:=clsT) (cls':=cls'). 
+        apply IHt1. auto. auto.  
+        apply heap_preserve_typing with (h:=h).
+          intros o0 cls_def0 F0 lo0. intro. 
+        apply reduction_preserve_heap_pointer with 
+                    (t:=(FieldWrite t1 i t2) )
+                     (s:=s) (s':=s') (h:=h) (h':=h')
+                                 (CT:=CT) (gamma:=gamma) (T:= T)
+                                  (t':=t') (F:=F0) (lo:=lo0); auto.
+        rewrite <- H.         rewrite <- H2. auto. auto.  auto. auto. 
+        
+        inversion typing. 
+        apply T_FieldWrite with (cls_def:=cls_def) (clsT:=clsT) (cls':=cls'). 
+        
+        apply heap_preserve_typing with (h:=h).
+          intros o0 cls_def0 F0 lo0. intro. 
+        apply reduction_preserve_heap_pointer with 
+                    (t:=(FieldWrite t1 i t2) )
+                     (s:=s) (s':=s') (h:=h) (h':=h')
+                                 (CT:=CT) (gamma:=gamma) (T:= T)
+                                  (t':=t') (F:=F0) (lo:=lo0); auto.
+        rewrite <- H.  rewrite <- H2. auto. auto.  auto. auto. auto.  
+
+        inversion typing. apply T_skip.         inversion typing. apply T_skip.
+
+(* if statement  *)
+   + intro T. intro typing. intro t'.  intro step.
+        inversion step. 
+        inversion typing. subst.  inversion H10. rewrite <- H3. auto.
+         inversion typing. subst. inversion H10. rewrite <- H3. auto.
+
+(* sequence *)
+   + intro T. intro typing. intro t'.  intro step.
+        inversion step. 
+        inversion typing. 
+        apply T_sequence with (T:=T0) (T':=T). 
+        apply IHt1. auto. auto.
+        apply heap_preserve_typing with (h:=h).
+          intros o0 cls_def0 F0 lo0. intro. 
+        apply reduction_preserve_heap_pointer with 
+                    (t:=(Sequence t1 t2)  )
+                     (s:=s) (s':=s') (h:=h) (h':=h')
+                                 (CT:=CT) (gamma:=gamma) (T:= T)
+                                  (t':=t') (F:=F0) (lo:=lo0); auto.
+        rewrite <- H.  rewrite <- H2. auto. auto.
+
+        inversion typing. rewrite <- H7.  
+        apply heap_preserve_typing with (h:=h).
+          intros o0 cls_def0 F0 lo0. intro. 
+        apply reduction_preserve_heap_pointer with 
+                    (t:=(Sequence t1 t2)  )
+                     (s:=s) (s':=s') (h:=h) (h':=h')
+                                 (CT:=CT) (gamma:=gamma) (T:= T)
+                                  (t':=t') (F:=F0) (lo:=lo0); auto.
+        rewrite <- H.  rewrite <- H2. auto. auto.
+
+(* return   *)
+   + intro T. intro typing. intro t'.  intro step.
+        inversion step. 
+        inversion typing. 
+        apply T_return. apply IHt.  auto. auto.  auto. 
+        
+        inversion typing. rewrite <- H5. 
+        apply heap_preserve_typing with (h:=h).
+          intros o0 cls_def0 F0 lo0. intro. 
+        apply reduction_preserve_heap_pointer with 
+                    (t:=(Return t) )
+                     (s:=s) (s':=s') (h:=h) (h':=h')
+                                 (CT:=CT) (gamma:=gamma) (T:= T)
+                                  (t':=t') (F:=F0) (lo:=lo0); auto.
+        rewrite <- H.  rewrite <- H2. auto. auto.
+
+(* objId *)
+     + intro T. intro typing. intro t'.  intro step.
+        inversion step. 
+
+(* runtime labeled data *)
+     + intro T. intro typing. intro t'.  intro step.
+        inversion step. 
+(* runtime opaque labeled data *)
+     + intro T. intro typing. intro t'.  intro step.
+        inversion step. 
+Qed. 
+
+Inductive multi_step_reduction : config -> config -> Prop := 
+  | multi_reduction_refl : forall config , multi_step_reduction config config
+  | multi_reduction_step : forall c1 c2 c3, 
+                    reduction c1 c2 ->
+                    multi_step_reduction c2 c3 ->
+                    multi_step_reduction c1 c3.
+
+Inductive multi_step : tm -> Sigma -> tm -> Sigma -> Prop := 
+  | multi_refl : forall t sigma , multi_step t sigma t sigma
+  | multi_reduction : forall t1 t2 t3 sigma1 sigma2 sigma3, 
+                    reduction (Config t1 sigma1) (Config t2 sigma2) ->
+                    multi_step t2 sigma2 t3 sigma3 ->
+                    multi_step t1 sigma1 t3 sigma3.
+
+Notation "c1 '==>*' c2" := (multi_step_reduction c1 c2) (at level 40).
 
 
+Theorem soundness : forall gamma CT,
+    forall sigma s h, sigma = SIGMA s h ->  wfe_heap CT gamma h -> wfe_stack CT gamma h s -> 
+    forall t s' h' t',  multi_step t sigma t' (SIGMA s' h')  ->
+    forall T, has_type CT gamma h t T -> 
+     value t' \/ (exists config', Config t' (SIGMA s' h') ==> config').
+Proof with auto. 
+  intros  gamma CT sigma s h.  intro. intro. intro. intros t s' h' t'.
+  intro multiH. 
 
+generalize dependent s.  generalize dependent h. 
+  induction multiH.
+  + intro h. intro well_heap. intro s. intro sigmaH. intro well_stack. intro T. 
+     intro typing. apply progress with  (T:=T) (gamma:=gamma) (CT:=CT)  (s:=s) (h:=h); auto.
+  + intro h1. intro well_heap. intro s1. intro. intro well_stack. intro T. intro typing. 
+      induction sigma2.  
+      assert (wfe_heap CT gamma h /\ wfe_stack CT gamma h s).
+      apply reduction_preserve_wfe with (t:=t1) (t':=t2) 
+              (sigma:=sigma1) (sigma':=(SIGMA s h)) (gamma:=gamma) (CT:=CT)
+              (s:=s1) (s':=s) (h:=h1) (h':=h) (T:=T).
+      auto. auto.       auto. auto.       auto. auto. 
+      destruct IHmultiH with (h0:=h) (s0:=s) (T:=T).
+      apply H1. auto. apply H1.
+      apply preservation with (gamma:=gamma) (CT:=CT) (s:=s1) (s':=s) 
+                    (h:=h1) (h':=h) (sigma:=sigma1) (sigma':= (SIGMA s h)) (t:=t1).
+      auto.       auto.       auto.       auto.       auto.       auto. 
+      left. auto. right. auto.
+Qed.
 
+Theorem deterministic: forall t sigma t1 sigma1 t2 sigma2, 
+     reduction (Config t sigma) (Config t1 sigma1) ->
+     reduction (Config t sigma) (Config t2 sigma2) -> 
+      t1 = t2 /\ sigma1 = sigma2. 
+Proof.
+     intros t sigma t1 sigma1 t2 sigma2 Hy1 Hy2.
+
+     remember (Config t1 sigma1) as _t1_config. 
+     generalize dependent t2.
+     induction Hy1; intros t2 Hy2. 
+      (*Tvar *)
+     + inversion Hy2. subst. inversion H6. rewrite <- H1 in H10. rewrite <- H2 in H10.
+        inversion H10. inversion  Heq_t1_config.
+          split. auto. auto. 
+     (*field access*)
+    + inversion Hy2. inversion Heq_t1_config. subst. 
+      
+Admitted. 
